Clean Earley_Recognizer

Earley_Recognizer.thy
@@ -105,34 +105,34 @@ definition bins_upto :: "'a bins \<Rightarrow> nat \<Rightarrow> nat \<Rightarro
   "bins_upto bs k i \<equiv> \<Union> { set (items (bs ! l)) | l. l < k } \<union> bin_upto (bs ! k) i"
 
 definition wf_bin_items :: "'a cfg \<Rightarrow> 'a sentence \<Rightarrow> nat \<Rightarrow> 'a item list \<Rightarrow> bool" where
-  "wf_bin_items cfg inp k xs \<equiv> \<forall>x \<in> set xs. wf_item cfg inp x \<and> item_end x = k"
+  "wf_bin_items \<G> \<omega> k xs \<equiv> \<forall>x \<in> set xs. wf_item \<G> \<omega> x \<and> item_end x = k"
 
 definition wf_bin :: "'a cfg \<Rightarrow> 'a sentence \<Rightarrow> nat \<Rightarrow> 'a bin \<Rightarrow> bool" where
-  "wf_bin cfg inp k b \<equiv> distinct (items b) \<and> wf_bin_items cfg inp k (items b)"
+  "wf_bin \<G> \<omega> k b \<equiv> distinct (items b) \<and> wf_bin_items \<G> \<omega> k (items b)"
 
 definition wf_bins :: "'a cfg \<Rightarrow> 'a list \<Rightarrow> 'a bins \<Rightarrow> bool" where
-  "wf_bins cfg inp bs \<equiv> \<forall>k < length bs. wf_bin cfg inp k (bs!k)"
+  "wf_bins \<G> \<omega> bs \<equiv> \<forall>k < length bs. wf_bin \<G> \<omega> k (bs!k)"
 
 definition nonempty_derives :: "'a cfg \<Rightarrow> bool" where
-  "nonempty_derives cfg \<equiv> \<forall>N. N \<in> set (\<NN> cfg) \<longrightarrow> \<not> derives cfg [N] []"
+  "nonempty_derives \<G> \<equiv> \<forall>N. N \<in> set (\<NN> \<G>) \<longrightarrow> \<not> derives \<G> [N] []"
 
 definition Init\<^sub>L :: "'a cfg \<Rightarrow> 'a sentence \<Rightarrow> 'a bins" where
-  "Init\<^sub>L cfg inp \<equiv>
-    let rs = filter (\<lambda>r. rule_head r = \<SS> cfg) (\<RR> cfg) in
+  "Init\<^sub>L \<G> \<omega> \<equiv>
+    let rs = filter (\<lambda>r. rule_head r = \<SS> \<G>) (\<RR> \<G>) in
     let b0 = map (\<lambda>r. (Entry (init_item r 0) Null)) rs in
-    let bs = replicate (length inp + 1) ([]) in
+    let bs = replicate (length \<omega> + 1) ([]) in
     bs[0 := b0]"
 
 definition Scan\<^sub>L :: "nat \<Rightarrow> 'a sentence \<Rightarrow> 'a  \<Rightarrow> 'a item \<Rightarrow> nat \<Rightarrow> 'a entry list" where
-  "Scan\<^sub>L k inp a x pre \<equiv>
-    if inp!k = a then
+  "Scan\<^sub>L k \<omega> a x pre \<equiv>
+    if \<omega>!k = a then
       let x' = inc_item x (k+1) in
       [Entry x' (Pre pre)]
     else []"
 
 definition Predict\<^sub>L :: "nat \<Rightarrow> 'a cfg \<Rightarrow> 'a \<Rightarrow> 'a entry list" where
-  "Predict\<^sub>L k cfg X \<equiv>
-    let rs = filter (\<lambda>r. rule_head r = X) (\<RR> cfg) in
+  "Predict\<^sub>L k \<G> X \<equiv>
+    let rs = filter (\<lambda>r. rule_head r = X) (\<RR> \<G>) in
     map (\<lambda>r. (Entry (init_item r k) Null)) rs"
 
 definition Complete\<^sub>L :: "nat \<Rightarrow> 'a item \<Rightarrow> 'a bins \<Rightarrow> nat \<Rightarrow> 'a entry list" where
@@ -160,31 +160,31 @@ definition bins_upd :: "'a bins \<Rightarrow> nat \<Rightarrow> 'a entry list \<
   "bins_upd bs k es \<equiv> bs[k := bin_upds es (bs!k)]"
 
 partial_function (tailrec) Earley\<^sub>L_bin' :: "nat \<Rightarrow> 'a cfg \<Rightarrow> 'a sentence \<Rightarrow> 'a bins \<Rightarrow> nat \<Rightarrow> 'a bins" where
-  "Earley\<^sub>L_bin' k cfg inp bs i = (
+  "Earley\<^sub>L_bin' k \<G> \<omega> bs i = (
     if i \<ge> length (items (bs ! k)) then bs
     else
       let x = items (bs!k) ! i in
       let bs' =
         case next_symbol x of
           Some a \<Rightarrow>
-            if is_terminal cfg a then
-              if k < length inp then bins_upd bs (k+1) (Scan\<^sub>L k inp a x i)
+            if is_terminal \<G> a then
+              if k < length \<omega> then bins_upd bs (k+1) (Scan\<^sub>L k \<omega> a x i)
               else bs
-            else bins_upd bs k (Predict\<^sub>L k cfg a)
+            else bins_upd bs k (Predict\<^sub>L k \<G> a)
         | None \<Rightarrow> bins_upd bs k (Complete\<^sub>L k x bs i)
-      in Earley\<^sub>L_bin' k cfg inp bs' (i+1))"
+      in Earley\<^sub>L_bin' k \<G> \<omega> bs' (i+1))"
 
 declare Earley\<^sub>L_bin'.simps[code]
 
 definition Earley\<^sub>L_bin :: "nat \<Rightarrow> 'a cfg \<Rightarrow> 'a sentence \<Rightarrow> 'a bins \<Rightarrow> 'a bins" where
-  "Earley\<^sub>L_bin k cfg inp bs \<equiv> Earley\<^sub>L_bin' k cfg inp bs 0"
+  "Earley\<^sub>L_bin k \<G> \<omega> bs \<equiv> Earley\<^sub>L_bin' k \<G> \<omega> bs 0"
 
 fun Earley\<^sub>L_bins :: "nat \<Rightarrow> 'a cfg \<Rightarrow> 'a sentence \<Rightarrow> 'a bins" where
-  "Earley\<^sub>L_bins 0 cfg inp = Earley\<^sub>L_bin 0 cfg inp (Init\<^sub>L cfg inp)"
-| "Earley\<^sub>L_bins (Suc n) cfg inp = Earley\<^sub>L_bin (Suc n) cfg inp (Earley\<^sub>L_bins n cfg inp)"
+  "Earley\<^sub>L_bins 0 \<G> \<omega> = Earley\<^sub>L_bin 0 \<G> \<omega> (Init\<^sub>L \<G> \<omega>)"
+| "Earley\<^sub>L_bins (Suc n) \<G> \<omega> = Earley\<^sub>L_bin (Suc n) \<G> \<omega> (Earley\<^sub>L_bins n \<G> \<omega>)"
 
 definition Earley\<^sub>L :: "'a cfg \<Rightarrow> 'a sentence \<Rightarrow> 'a bins" where
-  "Earley\<^sub>L cfg inp \<equiv> Earley\<^sub>L_bins (length inp) cfg inp"
+  "Earley\<^sub>L \<G> \<omega> \<equiv> Earley\<^sub>L_bins (length \<omega>) \<G> \<omega>"
 
 
 subsection \<open>Bin lemmas\<close>
@@ -409,12 +409,12 @@ proof (induction b arbitrary: e)
 qed (auto simp: items_def)
 
 lemma wf_bins_kth_bin:
-  "wf_bins cfg inp bs \<Longrightarrow> k < length bs \<Longrightarrow> x \<in> set (items (bs ! k)) \<Longrightarrow> wf_item cfg inp x \<and> item_end x = k"
+  "wf_bins \<G> \<omega> bs \<Longrightarrow> k < length bs \<Longrightarrow> x \<in> set (items (bs ! k)) \<Longrightarrow> wf_item \<G> \<omega> x \<and> item_end x = k"
   using wf_bin_def wf_bins_def wf_bin_items_def by blast
 
 lemma wf_bin_bin_upd:
-  assumes "wf_bin cfg inp k b" "wf_item cfg inp (item e) \<and> item_end (item e) = k"
-  shows "wf_bin cfg inp k (bin_upd e b)"
+  assumes "wf_bin \<G> \<omega> k b" "wf_item \<G> \<omega> (item e) \<and> item_end (item e) = k"
+  shows "wf_bin \<G> \<omega> k (bin_upd e b)"
   using assms
 proof (induction b arbitrary: e)
   case (Cons b bs)
@@ -447,20 +447,20 @@ proof (induction b arbitrary: e)
 qed (auto simp: items_def wf_bin_def wf_bin_items_def)
 
 lemma wf_bin_bin_upds:
-  assumes "wf_bin cfg inp k b" "distinct (items es)"
-  assumes "\<forall>x \<in> set (items es). wf_item cfg inp x \<and> item_end x = k"
-  shows "wf_bin cfg inp k (bin_upds es b)"
+  assumes "wf_bin \<G> \<omega> k b" "distinct (items es)"
+  assumes "\<forall>x \<in> set (items es). wf_item \<G> \<omega> x \<and> item_end x = k"
+  shows "wf_bin \<G> \<omega> k (bin_upds es b)"
   using assms by (induction es arbitrary: b) (auto simp: wf_bin_bin_upd items_def)
 
 lemma wf_bins_bins_upd:
-  assumes "wf_bins cfg inp bs" "distinct (items es)"
-  assumes "\<forall>x \<in> set (items es). wf_item cfg inp x \<and> item_end x = k"
-  shows "wf_bins cfg inp (bins_upd bs k es)"
+  assumes "wf_bins \<G> \<omega> bs" "distinct (items es)"
+  assumes "\<forall>x \<in> set (items es). wf_item \<G> \<omega> x \<and> item_end x = k"
+  shows "wf_bins \<G> \<omega> (bins_upd bs k es)"
   unfolding bins_upd_def using assms wf_bin_bin_upds wf_bins_def
   by (metis length_list_update nth_list_update_eq nth_list_update_neq)
 
 lemma wf_bins_impl_wf_items:
-  "wf_bins cfg inp bs \<Longrightarrow> \<forall>x \<in> (bins bs). wf_item cfg inp x"
+  "wf_bins \<G> \<omega> bs \<Longrightarrow> \<forall>x \<in> (bins bs). wf_item \<G> \<omega> x"
   unfolding wf_bins_def wf_bin_def wf_bin_items_def bins_def by auto
 
 lemma bin_upds_eq_items:
@@ -662,11 +662,11 @@ qed
 subsection \<open>Well-formed bins\<close>
 
 lemma distinct_Scan\<^sub>L:
-  "distinct (items (Scan\<^sub>L k inp a x pre))"
+  "distinct (items (Scan\<^sub>L k \<omega> a x pre))"
   unfolding Scan\<^sub>L_def by (auto simp: items_def)
 
 lemma distinct_Predict\<^sub>L:
-  "wf_\<G> cfg \<Longrightarrow> distinct (items (Predict\<^sub>L k cfg X))"
+  "wf_\<G> \<G> \<Longrightarrow> distinct (items (Predict\<^sub>L k \<G> X))"
   unfolding Predict\<^sub>L_def wf_\<G>_defs by (auto simp: init_item_def rule_head_def distinct_map inj_on_def items_def)
 
 lemma inj_on_inc_item:
@@ -674,13 +674,13 @@ lemma inj_on_inc_item:
   unfolding inj_on_def inc_item_def by (simp add: item.expand)
 
 lemma distinct_Complete\<^sub>L:
-  assumes "wf_bins cfg inp bs" "item_origin y < length bs"
+  assumes "wf_bins \<G> \<omega> bs" "item_origin y < length bs"
   shows "distinct (items (Complete\<^sub>L k y bs red))"
 proof -
   let ?orig = "bs ! (item_origin y)"
   let ?is = "filter_with_index (\<lambda>x. next_symbol x = Some (item_rule_head y)) (items ?orig)"
   let ?is' = "map (\<lambda>(x, pre). (Entry (inc_item x k) (PreRed (item_origin y, pre, red) []))) ?is"
-  have wf: "wf_bin cfg inp (item_origin y) ?orig"
+  have wf: "wf_bin \<G> \<omega> (item_origin y) ?orig"
     using assms wf_bins_def by blast
   have 0: "\<forall>x \<in> set (map fst ?is). item_end x = (item_origin y)"
     using wf wf_bin_def wf_bin_items_def filter_is_subset filter_with_index_cong_filter by (metis in_mono)
@@ -699,31 +699,31 @@ proof -
 qed
 
 lemma wf_bins_Scan\<^sub>L':
-  assumes "wf_bins cfg inp bs" "k < length bs" "x \<in> set (items (bs ! k))"
-  assumes "k < length inp" "next_symbol x \<noteq> None" "y = inc_item x (k+1)"
-  shows "wf_item cfg inp y \<and> item_end y = k+1"
+  assumes "wf_bins \<G> \<omega> bs" "k < length bs" "x \<in> set (items (bs ! k))"
+  assumes "k < length \<omega>" "next_symbol x \<noteq> None" "y = inc_item x (k+1)"
+  shows "wf_item \<G> \<omega> y \<and> item_end y = k+1"
   using assms wf_bins_kth_bin[OF assms(1-3)]
   unfolding wf_item_def inc_item_def next_symbol_def is_complete_def item_rule_body_def
   by (auto split: if_splits)
 
 lemma wf_bins_Scan\<^sub>L:
-  assumes "wf_bins cfg inp bs" "k < length bs" "x \<in> set (items (bs ! k))" "k < length inp" "next_symbol x \<noteq> None"
-  shows "\<forall>y \<in> set (items (Scan\<^sub>L k inp a x pre)). wf_item cfg inp y \<and> item_end y = (k+1)"
+  assumes "wf_bins \<G> \<omega> bs" "k < length bs" "x \<in> set (items (bs ! k))" "k < length \<omega>" "next_symbol x \<noteq> None"
+  shows "\<forall>y \<in> set (items (Scan\<^sub>L k \<omega> a x pre)). wf_item \<G> \<omega> y \<and> item_end y = (k+1)"
   using wf_bins_Scan\<^sub>L'[OF assms] by (simp add: Scan\<^sub>L_def items_def)
 
 lemma wf_bins_Predict\<^sub>L:
-  assumes "wf_bins cfg inp bs" "k < length bs" "k \<le> length inp" "wf_\<G> cfg"
-  shows "\<forall>y \<in> set (items (Predict\<^sub>L k cfg X)). wf_item cfg inp y \<and> item_end y = k"
+  assumes "wf_bins \<G> \<omega> bs" "k < length bs" "k \<le> length \<omega>" "wf_\<G> \<G>"
+  shows "\<forall>y \<in> set (items (Predict\<^sub>L k \<G> X)). wf_item \<G> \<omega> y \<and> item_end y = k"
   using assms by (auto simp: Predict\<^sub>L_def wf_item_def wf_bins_def wf_bin_def init_item_def wf_\<G>_defs items_def)
 
 lemma wf_item_inc_item:
-  assumes "wf_item cfg inp x" "next_symbol x = Some a" "item_origin x \<le> k" "k \<le> length inp"
-  shows "wf_item cfg inp (inc_item x k) \<and> item_end (inc_item x k) = k"
+  assumes "wf_item \<G> \<omega> x" "next_symbol x = Some a" "item_origin x \<le> k" "k \<le> length \<omega>"
+  shows "wf_item \<G> \<omega> (inc_item x k) \<and> item_end (inc_item x k) = k"
   using assms by (auto simp: wf_item_def inc_item_def item_rule_body_def next_symbol_def is_complete_def split: if_splits)
 
 lemma wf_bins_Complete\<^sub>L:
-  assumes "wf_bins cfg inp bs" "k < length bs" "y \<in> set (items (bs ! k))"
-  shows "\<forall>x \<in> set (items (Complete\<^sub>L k y bs red)). wf_item cfg inp x \<and> item_end x = k"
+  assumes "wf_bins \<G> \<omega> bs" "k < length bs" "y \<in> set (items (bs ! k))"
+  shows "\<forall>x \<in> set (items (Complete\<^sub>L k y bs red)). wf_item \<G> \<omega> x \<and> item_end x = k"
 proof -
   let ?orig = "bs ! (item_origin y)"
   let ?is = "filter_with_index (\<lambda>x. next_symbol x = Some (item_rule_head y)) (items ?orig)"
@@ -734,27 +734,27 @@ proof -
     have "item_end x = item_origin y"
       using * assms wf_bins_kth_bin wf_item_def filter_with_index_cong_filter
       by (metis dual_order.strict_trans2 filter_is_subset subsetD)
-    have "wf_item cfg inp x"
+    have "wf_item \<G> \<omega> x"
       using * assms wf_bins_kth_bin wf_item_def filter_with_index_cong_filter
       by (metis dual_order.strict_trans2 filter_is_subset subsetD)
     moreover have "next_symbol x = Some (item_rule_head y)"
       using * filter_set filter_with_index_cong_filter member_filter by metis
     moreover have "item_origin x \<le> k"
-      using \<open>item_end x = item_origin y\<close> \<open>wf_item cfg inp x\<close> assms wf_bins_kth_bin wf_item_def
+      using \<open>item_end x = item_origin y\<close> \<open>wf_item \<G> \<omega> x\<close> assms wf_bins_kth_bin wf_item_def
       by (metis dual_order.order_iff_strict dual_order.strict_trans1)
-    moreover have "k \<le> length inp"
+    moreover have "k \<le> length \<omega>"
       using assms wf_bins_kth_bin wf_item_def by blast
-    ultimately have "wf_item cfg inp (inc_item x k)" "item_end (inc_item x k) = k"
+    ultimately have "wf_item \<G> \<omega> (inc_item x k)" "item_end (inc_item x k) = k"
       by (simp_all add: wf_item_inc_item)
   }
-  hence "\<forall>x \<in> set (items ?is'). wf_item cfg inp x \<and> item_end x = k"
+  hence "\<forall>x \<in> set (items ?is'). wf_item \<G> \<omega> x \<and> item_end x = k"
     by (auto simp: items_def rev_image_eqI)
   thus ?thesis
     unfolding Complete\<^sub>L_def by presburger
 qed
 
 lemma Ex_wf_bins:
-  "\<exists>n bs inp cfg. n \<le> length inp \<and> length bs = Suc (length inp) \<and> wf_\<G> cfg \<and> wf_bins cfg inp bs"
+  "\<exists>n bs \<omega> \<G>. n \<le> length \<omega> \<and> length bs = Suc (length \<omega>) \<and> wf_\<G> \<G> \<and> wf_bins \<G> \<omega> bs"
   apply (rule exI[where x="0"])
   apply (rule exI[where x="[[]]"])
   apply (rule exI[where x="[]"])
@@ -763,11 +763,11 @@ lemma Ex_wf_bins:
 
 definition wf_earley_input :: "(nat \<times> 'a cfg \<times> 'a sentence \<times> 'a bins) set" where
   "wf_earley_input = {
-    (k, cfg, inp, bs) | k cfg inp bs.
-      k \<le> length inp \<and>
-      length bs = length inp + 1 \<and>
-      wf_\<G> cfg \<and>
-      wf_bins cfg inp bs
+    (k, \<G>, \<omega>, bs) | k \<G> \<omega> bs.
+      k \<le> length \<omega> \<and>
+      length bs = length \<omega> + 1 \<and>
+      wf_\<G> \<G> \<and>
+      wf_bins \<G> \<omega> bs
   }"
 
 typedef 'a wf_bins = "wf_earley_input::(nat \<times> 'a cfg \<times> 'a sentence \<times> 'a bins) set"
@@ -775,44 +775,44 @@ typedef 'a wf_bins = "wf_earley_input::(nat \<times> 'a cfg \<times> 'a sentence
   using Ex_wf_bins by (auto simp: wf_earley_input_def)
 
 lemma wf_earley_input_elim:
-  assumes "(k, cfg, inp, bs) \<in> wf_earley_input"
-  shows "k \<le> length inp \<and> k < length bs \<and> length bs = length inp + 1 \<and> wf_\<G> cfg \<and> wf_bins cfg inp bs"
+  assumes "(k, \<G>, \<omega>, bs) \<in> wf_earley_input"
+  shows "k \<le> length \<omega> \<and> k < length bs \<and> length bs = length \<omega> + 1 \<and> wf_\<G> \<G> \<and> wf_bins \<G> \<omega> bs"
   using assms(1) from_wf_bins wf_earley_input_def by (smt (verit) Suc_eq_plus1 less_Suc_eq_le mem_Collect_eq prod.sel(1) snd_conv)
 
 lemma wf_earley_input_intro:
-  assumes "k \<le> length inp" "length bs = length inp + 1" "wf_\<G> cfg" "wf_bins cfg inp bs"
-  shows "(k, cfg, inp, bs) \<in> wf_earley_input"
+  assumes "k \<le> length \<omega>" "length bs = length \<omega> + 1" "wf_\<G> \<G>" "wf_bins \<G> \<omega> bs"
+  shows "(k, \<G>, \<omega>, bs) \<in> wf_earley_input"
   by (simp add: assms wf_earley_input_def)
 
 lemma wf_earley_input_Complete\<^sub>L:
-  assumes "(k, cfg, inp, bs) \<in> wf_earley_input" "\<not> length (items (bs ! k)) \<le> i"
+  assumes "(k, \<G>, \<omega>, bs) \<in> wf_earley_input" "\<not> length (items (bs ! k)) \<le> i"
   assumes "x = items (bs ! k) ! i" "next_symbol x = None"
-  shows "(k, cfg, inp, bins_upd bs k (Complete\<^sub>L k x bs red)) \<in> wf_earley_input"
+  shows "(k, \<G>, \<omega>, bins_upd bs k (Complete\<^sub>L k x bs red)) \<in> wf_earley_input"
 proof -
-  have *: "k \<le> length inp" "length bs = length inp + 1" "wf_\<G> cfg" "wf_bins cfg inp bs"
+  have *: "k \<le> length \<omega>" "length bs = length \<omega> + 1" "wf_\<G> \<G>" "wf_bins \<G> \<omega> bs"
     using wf_earley_input_elim assms(1) by metis+
   have x: "x \<in> set (items (bs ! k))"
     using assms(2,3) by simp
   have "item_origin x < length bs"
     using x wf_bins_kth_bin *(1,2,4) wf_item_def
     by (metis One_nat_def add.right_neutral add_Suc_right dual_order.trans le_imp_less_Suc)
-  hence "wf_bins cfg inp (bins_upd bs k (Complete\<^sub>L k x bs red))"
+  hence "wf_bins \<G> \<omega> (bins_upd bs k (Complete\<^sub>L k x bs red))"
     using *(1,2,4) Suc_eq_plus1 distinct_Complete\<^sub>L le_imp_less_Suc wf_bins_Complete\<^sub>L wf_bins_bins_upd x by metis
   thus ?thesis
     by (simp add: *(1-3) wf_earley_input_def)
 qed
 
 lemma wf_earley_input_Scan\<^sub>L:
-  assumes "(k, cfg, inp, bs) \<in> wf_earley_input" "\<not> length (items (bs ! k)) \<le> i"
+  assumes "(k, \<G>, \<omega>, bs) \<in> wf_earley_input" "\<not> length (items (bs ! k)) \<le> i"
   assumes "x = items (bs ! k) ! i" "next_symbol x = Some a"
-  assumes "is_terminal cfg a" "k < length inp"
-  shows "(k, cfg, inp, bins_upd bs (k+1) (Scan\<^sub>L k inp a x pre)) \<in> wf_earley_input"
+  assumes "is_terminal \<G> a" "k < length \<omega>"
+  shows "(k, \<G>, \<omega>, bins_upd bs (k+1) (Scan\<^sub>L k \<omega> a x pre)) \<in> wf_earley_input"
 proof -
-  have *: "k \<le> length inp" "length bs = length inp + 1" "wf_\<G> cfg" "wf_bins cfg inp bs"
+  have *: "k \<le> length \<omega>" "length bs = length \<omega> + 1" "wf_\<G> \<G>" "wf_bins \<G> \<omega> bs"
     using wf_earley_input_elim assms(1) by metis+
   have x: "x \<in> set (items(bs ! k))"
     using assms(2,3) by simp
-  have "wf_bins cfg inp (bins_upd bs (k+1) (Scan\<^sub>L k inp a x pre))"
+  have "wf_bins \<G> \<omega> (bins_upd bs (k+1) (Scan\<^sub>L k \<omega> a x pre))"
     using * x assms(1,4,6) distinct_Scan\<^sub>L wf_bins_Scan\<^sub>L wf_bins_bins_upd wf_earley_input_elim
     by (metis option.discI)
   thus ?thesis
@@ -820,58 +820,58 @@ proof -
 qed
 
 lemma wf_earley_input_Predict\<^sub>L:
-  assumes "(k, cfg, inp, bs) \<in> wf_earley_input" "\<not> length (items (bs ! k)) \<le> i"
-  assumes "x = items (bs ! k) ! i" "next_symbol x = Some a" "\<not> is_terminal cfg a"
-  shows "(k, cfg, inp, bins_upd bs k (Predict\<^sub>L k cfg a)) \<in> wf_earley_input"
+  assumes "(k, \<G>, \<omega>, bs) \<in> wf_earley_input" "\<not> length (items (bs ! k)) \<le> i"
+  assumes "x = items (bs ! k) ! i" "next_symbol x = Some a" "\<not> is_terminal \<G> a"
+  shows "(k, \<G>, \<omega>, bins_upd bs k (Predict\<^sub>L k \<G> a)) \<in> wf_earley_input"
 proof -
-  have *: "k \<le> length inp" "length bs = length inp + 1" "wf_\<G> cfg" "wf_bins cfg inp bs"
+  have *: "k \<le> length \<omega>" "length bs = length \<omega> + 1" "wf_\<G> \<G>" "wf_bins \<G> \<omega> bs"
     using wf_earley_input_elim assms(1) by metis+
   have x: "x \<in> set (items (bs ! k))"
     using assms(2,3) by simp
-  hence "wf_bins cfg inp (bins_upd bs k (Predict\<^sub>L k cfg a))"
+  hence "wf_bins \<G> \<omega> (bins_upd bs k (Predict\<^sub>L k \<G> a))"
     using * x assms(1,4) distinct_Predict\<^sub>L wf_bins_Predict\<^sub>L wf_bins_bins_upd wf_earley_input_elim by metis
   thus ?thesis
     by (simp add: *(1-3) wf_earley_input_def)
 qed
 
 fun earley_measure :: "nat \<times> 'a cfg \<times> 'a sentence \<times> 'a bins \<Rightarrow> nat \<Rightarrow> nat" where
-  "earley_measure (k, cfg, inp, bs) i = card { x | x. wf_item cfg inp x \<and> item_end x = k } - i"
+  "earley_measure (k, \<G>, \<omega>, bs) i = card { x | x. wf_item \<G> \<omega> x \<and> item_end x = k } - i"
 
 lemma Earley\<^sub>L_bin'_simps[simp]:
-  "i \<ge> length (items (bs ! k)) \<Longrightarrow> Earley\<^sub>L_bin' k cfg inp bs i = bs"
+  "i \<ge> length (items (bs ! k)) \<Longrightarrow> Earley\<^sub>L_bin' k \<G> \<omega> bs i = bs"
   "\<not> i \<ge> length (items (bs ! k)) \<Longrightarrow> x = items (bs!k) ! i \<Longrightarrow> next_symbol x = None \<Longrightarrow>
-    Earley\<^sub>L_bin' k cfg inp bs i = Earley\<^sub>L_bin' k cfg inp (bins_upd bs k (Complete\<^sub>L k x bs i)) (i+1)"
+    Earley\<^sub>L_bin' k \<G> \<omega> bs i = Earley\<^sub>L_bin' k \<G> \<omega> (bins_upd bs k (Complete\<^sub>L k x bs i)) (i+1)"
   "\<not> i \<ge> length (items (bs ! k)) \<Longrightarrow> x = items (bs!k) ! i \<Longrightarrow> next_symbol x = Some a \<Longrightarrow>
-    is_terminal cfg a \<Longrightarrow> k < length inp \<Longrightarrow> Earley\<^sub>L_bin' k cfg inp bs i = Earley\<^sub>L_bin' k cfg inp (bins_upd bs (k+1) (Scan\<^sub>L k inp a x i)) (i+1)"
+    is_terminal \<G> a \<Longrightarrow> k < length \<omega> \<Longrightarrow> Earley\<^sub>L_bin' k \<G> \<omega> bs i = Earley\<^sub>L_bin' k \<G> \<omega> (bins_upd bs (k+1) (Scan\<^sub>L k \<omega> a x i)) (i+1)"
   "\<not> i \<ge> length (items (bs ! k)) \<Longrightarrow> x = items (bs!k) ! i \<Longrightarrow> next_symbol x = Some a \<Longrightarrow>
-    is_terminal cfg a \<Longrightarrow> \<not> k < length inp \<Longrightarrow> Earley\<^sub>L_bin' k cfg inp bs i = Earley\<^sub>L_bin' k cfg inp bs (i+1)"
+    is_terminal \<G> a \<Longrightarrow> \<not> k < length \<omega> \<Longrightarrow> Earley\<^sub>L_bin' k \<G> \<omega> bs i = Earley\<^sub>L_bin' k \<G> \<omega> bs (i+1)"
   "\<not> i \<ge> length (items (bs ! k)) \<Longrightarrow> x = items (bs!k) ! i \<Longrightarrow> next_symbol x = Some a \<Longrightarrow>
-    \<not> is_terminal cfg a \<Longrightarrow> Earley\<^sub>L_bin' k cfg inp bs i = Earley\<^sub>L_bin' k cfg inp (bins_upd bs k (Predict\<^sub>L k cfg a)) (i+1)"
+    \<not> is_terminal \<G> a \<Longrightarrow> Earley\<^sub>L_bin' k \<G> \<omega> bs i = Earley\<^sub>L_bin' k \<G> \<omega> (bins_upd bs k (Predict\<^sub>L k \<G> a)) (i+1)"
   by (subst Earley\<^sub>L_bin'.simps, simp)+
 
 lemma Earley\<^sub>L_bin'_induct[case_names Base Complete\<^sub>F Scan\<^sub>F Pass Predict\<^sub>F]:
-  assumes "(k, cfg, inp, bs) \<in> wf_earley_input"
-  assumes base: "\<And>k cfg inp bs i. i \<ge> length (items (bs ! k)) \<Longrightarrow> P k cfg inp bs i"
-  assumes complete: "\<And>k cfg inp bs i x. \<not> i \<ge> length (items (bs ! k)) \<Longrightarrow> x = items (bs ! k) ! i \<Longrightarrow>
-            next_symbol x = None \<Longrightarrow> P k cfg inp (bins_upd bs k (Complete\<^sub>L k x bs i)) (i+1) \<Longrightarrow> P k cfg inp bs i"
-  assumes scan: "\<And>k cfg inp bs i x a. \<not> i \<ge> length (items (bs ! k)) \<Longrightarrow> x = items (bs ! k) ! i \<Longrightarrow>
-            next_symbol x = Some a \<Longrightarrow> is_terminal cfg a \<Longrightarrow> k < length inp \<Longrightarrow>
-            P k cfg inp (bins_upd bs (k+1) (Scan\<^sub>L k inp a x i)) (i+1) \<Longrightarrow> P k cfg inp bs i"
-  assumes pass: "\<And>k cfg inp bs i x a. \<not> i \<ge> length (items (bs ! k)) \<Longrightarrow> x = items (bs ! k) ! i \<Longrightarrow>
-            next_symbol x = Some a \<Longrightarrow> is_terminal cfg a \<Longrightarrow> \<not> k < length inp \<Longrightarrow>
-            P k cfg inp bs (i+1) \<Longrightarrow> P k cfg inp bs i"
-  assumes predict: "\<And>k cfg inp bs i x a. \<not> i \<ge> length (items (bs ! k)) \<Longrightarrow> x = items (bs ! k) ! i \<Longrightarrow>
-            next_symbol x = Some a \<Longrightarrow> \<not> is_terminal cfg a \<Longrightarrow>
-            P k cfg inp (bins_upd bs k (Predict\<^sub>L k cfg a)) (i+1) \<Longrightarrow> P k cfg inp bs i"
-  shows "P k cfg inp bs i"
+  assumes "(k, \<G>, \<omega>, bs) \<in> wf_earley_input"
+  assumes base: "\<And>k \<G> \<omega> bs i. i \<ge> length (items (bs ! k)) \<Longrightarrow> P k \<G> \<omega> bs i"
+  assumes complete: "\<And>k \<G> \<omega> bs i x. \<not> i \<ge> length (items (bs ! k)) \<Longrightarrow> x = items (bs ! k) ! i \<Longrightarrow>
+            next_symbol x = None \<Longrightarrow> P k \<G> \<omega> (bins_upd bs k (Complete\<^sub>L k x bs i)) (i+1) \<Longrightarrow> P k \<G> \<omega> bs i"
+  assumes scan: "\<And>k \<G> \<omega> bs i x a. \<not> i \<ge> length (items (bs ! k)) \<Longrightarrow> x = items (bs ! k) ! i \<Longrightarrow>
+            next_symbol x = Some a \<Longrightarrow> is_terminal \<G> a \<Longrightarrow> k < length \<omega> \<Longrightarrow>
+            P k \<G> \<omega> (bins_upd bs (k+1) (Scan\<^sub>L k \<omega> a x i)) (i+1) \<Longrightarrow> P k \<G> \<omega> bs i"
+  assumes pass: "\<And>k \<G> \<omega> bs i x a. \<not> i \<ge> length (items (bs ! k)) \<Longrightarrow> x = items (bs ! k) ! i \<Longrightarrow>
+            next_symbol x = Some a \<Longrightarrow> is_terminal \<G> a \<Longrightarrow> \<not> k < length \<omega> \<Longrightarrow>
+            P k \<G> \<omega> bs (i+1) \<Longrightarrow> P k \<G> \<omega> bs i"
+  assumes predict: "\<And>k \<G> \<omega> bs i x a. \<not> i \<ge> length (items (bs ! k)) \<Longrightarrow> x = items (bs ! k) ! i \<Longrightarrow>
+            next_symbol x = Some a \<Longrightarrow> \<not> is_terminal \<G> a \<Longrightarrow>
+            P k \<G> \<omega> (bins_upd bs k (Predict\<^sub>L k \<G> a)) (i+1) \<Longrightarrow> P k \<G> \<omega> bs i"
+  shows "P k \<G> \<omega> bs i"
   using assms(1)
-proof (induction n\<equiv>"earley_measure (k, cfg, inp, bs) i" arbitrary: bs i rule: nat_less_induct)
+proof (induction n\<equiv>"earley_measure (k, \<G>, \<omega>, bs) i" arbitrary: bs i rule: nat_less_induct)
   case 1
-  have wf: "k \<le> length inp" "length bs = length inp + 1" "wf_\<G> cfg" "wf_bins cfg inp bs"
+  have wf: "k \<le> length \<omega>" "length bs = length \<omega> + 1" "wf_\<G> \<G>" "wf_bins \<G> \<omega> bs"
     using "1.prems" wf_earley_input_elim by metis+
   hence k: "k < length bs"
     by simp
-  have fin: "finite { x | x. wf_item cfg inp x \<and> item_end x = k }"
+  have fin: "finite { x | x. wf_item \<G> \<omega> x \<and> item_end x = k }"
     using finiteness_UNIV_wf_item by fastforce
   show ?case
   proof cases
@@ -889,21 +889,21 @@ proof (induction n\<equiv>"earley_measure (k, cfg, inp, bs) i" arbitrary: bs i r
       let ?bs' = "bins_upd bs k (Complete\<^sub>L k ?x bs i)"
       have "item_origin ?x < length bs"
         using wf(4) k wf_bins_kth_bin wf_item_def x by (metis order_le_less_trans)
-      hence wf_bins': "wf_bins cfg inp ?bs'"
+      hence wf_bins': "wf_bins \<G> \<omega> ?bs'"
         using wf_bins_Complete\<^sub>L distinct_Complete\<^sub>L wf(4) wf_bins_bins_upd k x by metis
-      hence wf': "(k, cfg, inp, ?bs') \<in> wf_earley_input"
+      hence wf': "(k, \<G>, \<omega>, ?bs') \<in> wf_earley_input"
         using wf(1,2,3) wf_earley_input_intro by fastforce
-      have sub: "set (items (?bs' ! k)) \<subseteq> { x | x. wf_item cfg inp x \<and> item_end x = k }"
+      have sub: "set (items (?bs' ! k)) \<subseteq> { x | x. wf_item \<G> \<omega> x \<and> item_end x = k }"
         using wf(1,2) wf_bins' unfolding wf_bin_def wf_bins_def wf_bin_items_def using order_le_less_trans by auto
       have "i < length (items (?bs' ! k))"
         using a1 by (metis dual_order.strict_trans1 items_def leI length_map length_nth_bin_bins_upd)
       also have "... = card (set (items (?bs' ! k)))"
         using wf(1,2) wf_bins' distinct_card wf_bins_def wf_bin_def by (metis k length_bins_upd)
-      also have "... \<le> card {x |x. wf_item cfg inp x \<and> item_end x = k}"
+      also have "... \<le> card {x |x. wf_item \<G> \<omega> x \<and> item_end x = k}"
         using card_mono fin sub by blast
-      finally have "card {x |x. wf_item cfg inp x \<and> item_end x = k} > i"
+      finally have "card {x |x. wf_item \<G> \<omega> x \<and> item_end x = k} > i"
         by blast
-      hence "earley_measure (k, cfg, inp, ?bs') (Suc i) < earley_measure (k, cfg, inp, bs) i"
+      hence "earley_measure (k, \<G>, \<omega>, ?bs') (Suc i) < earley_measure (k, \<G>, \<omega>, bs) i"
         by simp
       thus ?thesis
         using 1 a1 a2 complete wf' by simp
@@ -913,66 +913,66 @@ proof (induction n\<equiv>"earley_measure (k, cfg, inp, bs) i" arbitrary: bs i r
         by blast
       show ?thesis
       proof cases
-        assume a3: "is_terminal cfg a"
+        assume a3: "is_terminal \<G> a"
         show ?thesis
         proof cases
-          assume a4: "k < length inp"
-          let ?bs' = "bins_upd bs (k+1) (Scan\<^sub>L k inp a ?x i)"
-          have wf_bins': "wf_bins cfg inp ?bs'"
+          assume a4: "k < length \<omega>"
+          let ?bs' = "bins_upd bs (k+1) (Scan\<^sub>L k \<omega> a ?x i)"
+          have wf_bins': "wf_bins \<G> \<omega> ?bs'"
             using wf_bins_Scan\<^sub>L distinct_Scan\<^sub>L wf(1,4) wf_bins_bins_upd a2 a4 k x by metis
-          hence wf': "(k, cfg, inp, ?bs') \<in> wf_earley_input"
+          hence wf': "(k, \<G>, \<omega>, ?bs') \<in> wf_earley_input"
             using wf(1,2,3) wf_earley_input_intro by fastforce
-          have sub: "set (items (?bs' ! k)) \<subseteq> { x | x. wf_item cfg inp x \<and> item_end x = k }"
+          have sub: "set (items (?bs' ! k)) \<subseteq> { x | x. wf_item \<G> \<omega> x \<and> item_end x = k }"
             using wf(1,2) wf_bins' unfolding wf_bin_def wf_bins_def wf_bin_items_def using order_le_less_trans by auto
           have "i < length (items (?bs' ! k))"
             using a1 by (metis dual_order.strict_trans1 items_def leI length_map length_nth_bin_bins_upd)
           also have "... = card (set (items (?bs' ! k)))"
             using wf(1,2) wf_bins' distinct_card wf_bins_def wf_bin_def
             by (metis Suc_eq_plus1 le_imp_less_Suc length_bins_upd)
-          also have "... \<le> card {x |x. wf_item cfg inp x \<and> item_end x = k}"
+          also have "... \<le> card {x |x. wf_item \<G> \<omega> x \<and> item_end x = k}"
             using card_mono fin sub by blast
-          finally have "card {x |x. wf_item cfg inp x \<and> item_end x = k} > i"
+          finally have "card {x |x. wf_item \<G> \<omega> x \<and> item_end x = k} > i"
             by blast
-          hence "earley_measure (k, cfg, inp, ?bs') (Suc i) < earley_measure (k, cfg, inp, bs) i"
+          hence "earley_measure (k, \<G>, \<omega>, ?bs') (Suc i) < earley_measure (k, \<G>, \<omega>, bs) i"
             by simp
           thus ?thesis
             using 1 a1 a_def a3 a4 scan wf' by simp
         next
-          assume a4: "\<not> k < length inp"
-          have sub: "set (items (bs ! k)) \<subseteq> { x | x. wf_item cfg inp x \<and> item_end x = k }"
+          assume a4: "\<not> k < length \<omega>"
+          have sub: "set (items (bs ! k)) \<subseteq> { x | x. wf_item \<G> \<omega> x \<and> item_end x = k }"
             using wf(1,2,4) unfolding wf_bin_def wf_bins_def wf_bin_items_def using order_le_less_trans by auto
           have "i < length (items (bs ! k))"
             using a1 by simp
           also have "... = card (set (items (bs ! k)))"
             using wf(1,2,4) distinct_card wf_bins_def wf_bin_def by (metis Suc_eq_plus1 le_imp_less_Suc)
-          also have "... \<le> card {x |x. wf_item cfg inp x \<and> item_end x = k}"
+          also have "... \<le> card {x |x. wf_item \<G> \<omega> x \<and> item_end x = k}"
             using card_mono fin sub by blast
-          finally have "card {x |x. wf_item cfg inp x \<and> item_end x = k} > i"
+          finally have "card {x |x. wf_item \<G> \<omega> x \<and> item_end x = k} > i"
             by blast
-          hence "earley_measure (k, cfg, inp, bs) (Suc i) < earley_measure (k, cfg, inp, bs) i"
+          hence "earley_measure (k, \<G>, \<omega>, bs) (Suc i) < earley_measure (k, \<G>, \<omega>, bs) i"
             by simp
           thus ?thesis
             using 1 a1 a3 a4 a_def pass by simp
         qed
       next
-        assume a3: "\<not> is_terminal cfg a"
-        let ?bs' = "bins_upd bs k (Predict\<^sub>L k cfg a)"
-        have wf_bins': "wf_bins cfg inp ?bs'"
+        assume a3: "\<not> is_terminal \<G> a"
+        let ?bs' = "bins_upd bs k (Predict\<^sub>L k \<G> a)"
+        have wf_bins': "wf_bins \<G> \<omega> ?bs'"
           using wf_bins_Predict\<^sub>L distinct_Predict\<^sub>L wf(1,3,4) wf_bins_bins_upd k x by metis
-        hence wf': "(k, cfg, inp, ?bs') \<in> wf_earley_input"
+        hence wf': "(k, \<G>, \<omega>, ?bs') \<in> wf_earley_input"
           using wf(1,2,3) wf_earley_input_intro by fastforce
-        have sub: "set (items (?bs' ! k)) \<subseteq> { x | x. wf_item cfg inp x \<and> item_end x = k }"
+        have sub: "set (items (?bs' ! k)) \<subseteq> { x | x. wf_item \<G> \<omega> x \<and> item_end x = k }"
           using wf(1,2) wf_bins' unfolding wf_bin_def wf_bins_def wf_bin_items_def using order_le_less_trans by auto
         have "i < length (items (?bs' ! k))"
           using a1 by (metis dual_order.strict_trans1 items_def leI length_map length_nth_bin_bins_upd)
         also have "... = card (set (items (?bs' ! k)))"
           using wf(1,2) wf_bins' distinct_card wf_bins_def wf_bin_def
           by (metis Suc_eq_plus1 le_imp_less_Suc length_bins_upd)
-        also have "... \<le> card {x |x. wf_item cfg inp x \<and> item_end x = k}"
+        also have "... \<le> card {x |x. wf_item \<G> \<omega> x \<and> item_end x = k}"
           using card_mono fin sub by blast
-        finally have "card {x |x. wf_item cfg inp x \<and> item_end x = k} > i"
+        finally have "card {x |x. wf_item \<G> \<omega> x \<and> item_end x = k} > i"
           by blast
-        hence "earley_measure (k, cfg, inp, ?bs') (Suc i) < earley_measure (k, cfg, inp, bs) i"
+        hence "earley_measure (k, \<G>, \<omega>, ?bs') (Suc i) < earley_measure (k, \<G>, \<omega>, bs) i"
           by simp
         thus ?thesis
           using 1 a1 a_def a3 a_def predict wf' by simp
@@ -982,85 +982,85 @@ proof (induction n\<equiv>"earley_measure (k, cfg, inp, bs) i" arbitrary: bs i r
 qed
 
 lemma wf_earley_input_Earley\<^sub>L_bin':
-  assumes "(k, cfg, inp, bs) \<in> wf_earley_input"
-  shows "(k, cfg, inp, Earley\<^sub>L_bin' k cfg inp bs i) \<in> wf_earley_input"
+  assumes "(k, \<G>, \<omega>, bs) \<in> wf_earley_input"
+  shows "(k, \<G>, \<omega>, Earley\<^sub>L_bin' k \<G> \<omega> bs i) \<in> wf_earley_input"
   using assms
 proof (induction i rule: Earley\<^sub>L_bin'_induct[OF assms(1), case_names Base Complete\<^sub>F Scan\<^sub>F Pass Predict\<^sub>F])
-  case (Complete\<^sub>F k cfg inp bs i x)
+  case (Complete\<^sub>F k \<G> \<omega> bs i x)
   let ?bs' = "bins_upd bs k (Complete\<^sub>L k x bs i)"
-  have "(k, cfg, inp, ?bs') \<in> wf_earley_input"
+  have "(k, \<G>, \<omega>, ?bs') \<in> wf_earley_input"
     using Complete\<^sub>F.hyps Complete\<^sub>F.prems wf_earley_input_Complete\<^sub>L by blast
   thus ?case
     using Complete\<^sub>F.IH Complete\<^sub>F.hyps by simp
 next
-  case (Scan\<^sub>F k cfg inp bs i x a)
-  let ?bs' = "bins_upd bs (k+1) (Scan\<^sub>L k inp a x i)"
-  have "(k, cfg, inp, ?bs') \<in> wf_earley_input"
+  case (Scan\<^sub>F k \<G> \<omega> bs i x a)
+  let ?bs' = "bins_upd bs (k+1) (Scan\<^sub>L k \<omega> a x i)"
+  have "(k, \<G>, \<omega>, ?bs') \<in> wf_earley_input"
     using Scan\<^sub>F.hyps Scan\<^sub>F.prems wf_earley_input_Scan\<^sub>L by metis
   thus ?case
     using Scan\<^sub>F.IH Scan\<^sub>F.hyps by simp
 next
-  case (Predict\<^sub>F k cfg inp bs i x a)
-  let ?bs' = "bins_upd bs k (Predict\<^sub>L k cfg a)"
-  have "(k, cfg, inp, ?bs') \<in> wf_earley_input"
+  case (Predict\<^sub>F k \<G> \<omega> bs i x a)
+  let ?bs' = "bins_upd bs k (Predict\<^sub>L k \<G> a)"
+  have "(k, \<G>, \<omega>, ?bs') \<in> wf_earley_input"
     using Predict\<^sub>F.hyps Predict\<^sub>F.prems wf_earley_input_Predict\<^sub>L by metis
   thus ?case
     using Predict\<^sub>F.IH Predict\<^sub>F.hyps by simp
 qed simp_all
 
 lemma wf_earley_input_Earley\<^sub>L_bin:
-  assumes "(k, cfg, inp, bs) \<in> wf_earley_input"
-  shows "(k, cfg, inp, Earley\<^sub>L_bin k cfg inp bs) \<in> wf_earley_input"
+  assumes "(k, \<G>, \<omega>, bs) \<in> wf_earley_input"
+  shows "(k, \<G>, \<omega>, Earley\<^sub>L_bin k \<G> \<omega> bs) \<in> wf_earley_input"
   using assms by (simp add: Earley\<^sub>L_bin_def wf_earley_input_Earley\<^sub>L_bin')
 
 lemma length_bins_Earley\<^sub>L_bin':
-  assumes "(k, cfg, inp, bs) \<in> wf_earley_input"
-  shows "length (Earley\<^sub>L_bin' k cfg inp bs i) = length bs"
+  assumes "(k, \<G>, \<omega>, bs) \<in> wf_earley_input"
+  shows "length (Earley\<^sub>L_bin' k \<G> \<omega> bs i) = length bs"
   by (metis assms wf_earley_input_Earley\<^sub>L_bin' wf_earley_input_elim)
 
 lemma length_nth_bin_Earley\<^sub>L_bin':
-  assumes "(k, cfg, inp, bs) \<in> wf_earley_input"
-  shows "length (items (Earley\<^sub>L_bin' k cfg inp bs i ! l)) \<ge> length (items (bs ! l))"
+  assumes "(k, \<G>, \<omega>, bs) \<in> wf_earley_input"
+  shows "length (items (Earley\<^sub>L_bin' k \<G> \<omega> bs i ! l)) \<ge> length (items (bs ! l))"
   using length_nth_bin_bins_upd order_trans
   by (induction i rule: Earley\<^sub>L_bin'_induct[OF assms]) (auto simp: items_def, blast+)
 
 lemma wf_bins_Earley\<^sub>L_bin':
-  assumes "(k, cfg, inp, bs) \<in> wf_earley_input"
-  shows "wf_bins cfg inp (Earley\<^sub>L_bin' k cfg inp bs i)"
+  assumes "(k, \<G>, \<omega>, bs) \<in> wf_earley_input"
+  shows "wf_bins \<G> \<omega> (Earley\<^sub>L_bin' k \<G> \<omega> bs i)"
   using assms wf_earley_input_Earley\<^sub>L_bin' wf_earley_input_elim by blast
 
 lemma wf_bins_Earley\<^sub>L_bin:
-  assumes "(k, cfg, inp, bs) \<in> wf_earley_input"
-  shows "wf_bins cfg inp (Earley\<^sub>L_bin k cfg inp bs)"
+  assumes "(k, \<G>, \<omega>, bs) \<in> wf_earley_input"
+  shows "wf_bins \<G> \<omega> (Earley\<^sub>L_bin k \<G> \<omega> bs)"
   using assms Earley\<^sub>L_bin_def wf_bins_Earley\<^sub>L_bin' by metis
 
 lemma kth_Earley\<^sub>L_bin'_bins:
-  assumes "(k, cfg, inp, bs) \<in> wf_earley_input"
+  assumes "(k, \<G>, \<omega>, bs) \<in> wf_earley_input"
   assumes "j < length (items (bs ! l))"
-  shows "items (Earley\<^sub>L_bin' k cfg inp bs i ! l) ! j = items (bs ! l) ! j"
+  shows "items (Earley\<^sub>L_bin' k \<G> \<omega> bs i ! l) ! j = items (bs ! l) ! j"
   using assms(2)
 proof (induction i rule: Earley\<^sub>L_bin'_induct[OF assms(1), case_names Base Complete\<^sub>F Scan\<^sub>F Pass Predict\<^sub>F])
-  case (Complete\<^sub>F k cfg inp bs i x)
+  case (Complete\<^sub>F k \<G> \<omega> bs i x)
   let ?bs' = "bins_upd bs k (Complete\<^sub>L k x bs i)"
-  have "items (Earley\<^sub>L_bin' k cfg inp ?bs' (i + 1) ! l) ! j = items (?bs' ! l) ! j"
+  have "items (Earley\<^sub>L_bin' k \<G> \<omega> ?bs' (i + 1) ! l) ! j = items (?bs' ! l) ! j"
     using Complete\<^sub>F.IH Complete\<^sub>F.prems length_nth_bin_bins_upd items_def order.strict_trans2 by (metis length_map)
   also have "... = items (bs ! l) ! j"
     using Complete\<^sub>F.prems items_nth_idem_bins_upd nth_idem_bins_upd length_map items_def by metis
   finally show ?case
     using Complete\<^sub>F.hyps by simp
 next
-  case (Scan\<^sub>F k cfg inp bs i x a)
-  let ?bs' = "bins_upd bs (k+1) (Scan\<^sub>L k inp a x i)"
-  have "items (Earley\<^sub>L_bin' k cfg inp ?bs' (i + 1) ! l) ! j = items (?bs' ! l) ! j"
+  case (Scan\<^sub>F k \<G> \<omega> bs i x a)
+  let ?bs' = "bins_upd bs (k+1) (Scan\<^sub>L k \<omega> a x i)"
+  have "items (Earley\<^sub>L_bin' k \<G> \<omega> ?bs' (i + 1) ! l) ! j = items (?bs' ! l) ! j"
     using Scan\<^sub>F.IH Scan\<^sub>F.prems length_nth_bin_bins_upd order.strict_trans2 items_def by (metis length_map)
   also have "... = items (bs ! l) ! j"
     using Scan\<^sub>F.prems items_nth_idem_bins_upd nth_idem_bins_upd length_map items_def by metis
   finally show ?case
     using Scan\<^sub>F.hyps by simp
 next
-  case (Predict\<^sub>F k cfg inp bs i x a)
-  let ?bs' = "bins_upd bs k (Predict\<^sub>L k cfg a)"
-  have "items (Earley\<^sub>L_bin' k cfg inp ?bs' (i + 1) ! l) ! j = items (?bs' ! l) ! j"
+  case (Predict\<^sub>F k \<G> \<omega> bs i x a)
+  let ?bs' = "bins_upd bs k (Predict\<^sub>L k \<G> a)"
+  have "items (Earley\<^sub>L_bin' k \<G> \<omega> ?bs' (i + 1) ! l) ! j = items (?bs' ! l) ! j"
     using Predict\<^sub>F.IH Predict\<^sub>F.prems length_nth_bin_bins_upd order.strict_trans2 items_def by (metis length_map)
   also have "... = items (bs ! l) ! j"
     using Predict\<^sub>F.prems items_nth_idem_bins_upd nth_idem_bins_upd length_map items_def by metis
@@ -1069,49 +1069,49 @@ next
 qed simp_all
 
 lemma nth_bin_sub_Earley\<^sub>L_bin':
-  assumes "(k, cfg, inp, bs) \<in> wf_earley_input"
-  shows "set (items (bs ! l)) \<subseteq> set (items (Earley\<^sub>L_bin' k cfg inp bs i ! l))"
+  assumes "(k, \<G>, \<omega>, bs) \<in> wf_earley_input"
+  shows "set (items (bs ! l)) \<subseteq> set (items (Earley\<^sub>L_bin' k \<G> \<omega> bs i ! l))"
 proof standard
   fix x
   assume "x \<in> set (items (bs ! l))"
   then obtain j where *: "j < length (items (bs ! l))" "items (bs ! l) ! j = x"
     using in_set_conv_nth by metis
-  have "x = items (Earley\<^sub>L_bin' k cfg inp bs i ! l) ! j"
+  have "x = items (Earley\<^sub>L_bin' k \<G> \<omega> bs i ! l) ! j"
     using kth_Earley\<^sub>L_bin'_bins assms * by metis
-  moreover have "j < length (items (Earley\<^sub>L_bin' k cfg inp bs i ! l))"
+  moreover have "j < length (items (Earley\<^sub>L_bin' k \<G> \<omega> bs i ! l))"
     using assms *(1) length_nth_bin_Earley\<^sub>L_bin' less_le_trans by blast
-  ultimately show "x \<in> set (items (Earley\<^sub>L_bin' k cfg inp bs i ! l))"
+  ultimately show "x \<in> set (items (Earley\<^sub>L_bin' k \<G> \<omega> bs i ! l))"
     by simp
 qed
 
 lemma nth_Earley\<^sub>L_bin'_eq:
-  assumes "(k, cfg, inp, bs) \<in> wf_earley_input"
-  shows "l < k \<Longrightarrow> Earley\<^sub>L_bin' k cfg inp bs i ! l = bs ! l"
+  assumes "(k, \<G>, \<omega>, bs) \<in> wf_earley_input"
+  shows "l < k \<Longrightarrow> Earley\<^sub>L_bin' k \<G> \<omega> bs i ! l = bs ! l"
   by (induction i rule: Earley\<^sub>L_bin'_induct[OF assms]) (auto simp: bins_upd_def)
 
 lemma set_items_Earley\<^sub>L_bin'_eq:
-  assumes "(k, cfg, inp, bs) \<in> wf_earley_input"
-  shows "l < k \<Longrightarrow> set (items (Earley\<^sub>L_bin' k cfg inp bs i ! l)) = set (items (bs ! l))"
+  assumes "(k, \<G>, \<omega>, bs) \<in> wf_earley_input"
+  shows "l < k \<Longrightarrow> set (items (Earley\<^sub>L_bin' k \<G> \<omega> bs i ! l)) = set (items (bs ! l))"
   by (simp add: assms nth_Earley\<^sub>L_bin'_eq)
 
 lemma bins_upto_k0_Earley\<^sub>L_bin'_eq:
-  assumes "(k, cfg, inp, bs) \<in> wf_earley_input"
-  shows "bins_upto (Earley\<^sub>L_bin k cfg inp bs) k 0 = bins_upto bs k 0"
+  assumes "(k, \<G>, \<omega>, bs) \<in> wf_earley_input"
+  shows "bins_upto (Earley\<^sub>L_bin k \<G> \<omega> bs) k 0 = bins_upto bs k 0"
   unfolding bins_upto_def bin_upto_def Earley\<^sub>L_bin_def using set_items_Earley\<^sub>L_bin'_eq assms nth_Earley\<^sub>L_bin'_eq by fastforce
 
 lemma wf_earley_input_Init\<^sub>L:
-  assumes "k \<le> length inp" "wf_\<G> cfg"
-  shows "(k, cfg, inp, Init\<^sub>L cfg inp) \<in> wf_earley_input"
+  assumes "k \<le> length \<omega>" "wf_\<G> \<G>"
+  shows "(k, \<G>, \<omega>, Init\<^sub>L \<G> \<omega>) \<in> wf_earley_input"
 proof -
-  let ?rs = "filter (\<lambda>r. rule_head r = \<SS> cfg) (\<RR> cfg)"
+  let ?rs = "filter (\<lambda>r. rule_head r = \<SS> \<G>) (\<RR> \<G>)"
   let ?b0 = "map (\<lambda>r. (Entry (init_item r 0) Null)) ?rs"
-  let ?bs = "replicate (length inp + 1) ([])"
+  let ?bs = "replicate (length \<omega> + 1) ([])"
   have "distinct (items ?b0)"
     using assms unfolding wf_bin_def wf_item_def wf_\<G>_def distinct_rules_def items_def
     by (auto simp: init_item_def distinct_map inj_on_def)
-  moreover have "\<forall>x \<in> set (items ?b0). wf_item cfg inp x \<and> item_end x = 0"
+  moreover have "\<forall>x \<in> set (items ?b0). wf_item \<G> \<omega> x \<and> item_end x = 0"
     using assms unfolding wf_bin_def wf_item_def by (auto simp: init_item_def items_def)
-  moreover have "wf_bins cfg inp ?bs"
+  moreover have "wf_bins \<G> \<omega> ?bs"
     unfolding wf_bins_def wf_bin_def wf_bin_items_def items_def using less_Suc_eq_0_disj by force
   ultimately show ?thesis
     using assms length_replicate wf_earley_input_intro
@@ -1120,50 +1120,50 @@ proof -
 qed
 
 lemma length_bins_Init\<^sub>L[simp]:
-  "length (Init\<^sub>L cfg inp) = length inp + 1"
+  "length (Init\<^sub>L \<G> \<omega>) = length \<omega> + 1"
   by (simp add: Init\<^sub>L_def)
 
 lemma wf_earley_input_Earley\<^sub>L_bins[simp]:
-  assumes "k \<le> length inp" "wf_\<G> cfg"
-  shows "(k, cfg, inp, Earley\<^sub>L_bins k cfg inp) \<in> wf_earley_input"
+  assumes "k \<le> length \<omega>" "wf_\<G> \<G>"
+  shows "(k, \<G>, \<omega>, Earley\<^sub>L_bins k \<G> \<omega>) \<in> wf_earley_input"
   using assms
 proof (induction k)
   case 0
-  have "(k, cfg, inp, Init\<^sub>L cfg inp) \<in> wf_earley_input"
+  have "(k, \<G>, \<omega>, Init\<^sub>L \<G> \<omega>) \<in> wf_earley_input"
     using assms wf_earley_input_Init\<^sub>L by blast
   thus ?case
     by (simp add: assms(2) wf_earley_input_Init\<^sub>L wf_earley_input_Earley\<^sub>L_bin)
 next
   case (Suc k)
-  have "(Suc k, cfg, inp, Earley\<^sub>L_bins k cfg inp) \<in> wf_earley_input"
+  have "(Suc k, \<G>, \<omega>, Earley\<^sub>L_bins k \<G> \<omega>) \<in> wf_earley_input"
     using Suc.IH Suc.prems(1) Suc_leD assms(2) wf_earley_input_elim wf_earley_input_intro by metis
   thus ?case
     by (simp add: wf_earley_input_Earley\<^sub>L_bin)
 qed
 
 lemma length_Earley\<^sub>L_bins[simp]:
-  assumes "k \<le> length inp" "wf_\<G> cfg"
-  shows "length (Earley\<^sub>L_bins k cfg inp) = length (Init\<^sub>L cfg inp)"
+  assumes "k \<le> length \<omega>" "wf_\<G> \<G>"
+  shows "length (Earley\<^sub>L_bins k \<G> \<omega>) = length (Init\<^sub>L \<G> \<omega>)"
   using assms wf_earley_input_Earley\<^sub>L_bins wf_earley_input_elim by fastforce
 
 lemma wf_bins_Earley\<^sub>L_bins[simp]:
-  assumes "k \<le> length inp" "wf_\<G> cfg"
-  shows "wf_bins cfg inp (Earley\<^sub>L_bins k cfg inp)"
+  assumes "k \<le> length \<omega>" "wf_\<G> \<G>"
+  shows "wf_bins \<G> \<omega> (Earley\<^sub>L_bins k \<G> \<omega>)"
   using assms wf_earley_input_Earley\<^sub>L_bins wf_earley_input_elim by fastforce
 
 lemma wf_bins_Earley\<^sub>L:
-  "wf_\<G> cfg \<Longrightarrow> wf_bins cfg inp (Earley\<^sub>L cfg inp)"
+  "wf_\<G> \<G> \<Longrightarrow> wf_bins \<G> \<omega> (Earley\<^sub>L \<G> \<omega>)"
   by (simp add: Earley\<^sub>L_def)
 
 
-subsection \<open>List to set\<close>
+subsection \<open>Soundness\<close>
 
 lemma Init\<^sub>L_eq_Init\<^sub>F:
-  "bins (Init\<^sub>L cfg inp) = Init\<^sub>F cfg"
+  "bins (Init\<^sub>L \<G> \<omega>) = Init\<^sub>F \<G>"
 proof -
-  let ?rs = "filter (\<lambda>r. rule_head r = \<SS> cfg) (\<RR> cfg)"
+  let ?rs = "filter (\<lambda>r. rule_head r = \<SS> \<G>) (\<RR> \<G>)"
   let ?b0 = "map (\<lambda>r. (Entry (init_item r 0) Null)) ?rs"
-  let ?bs = "replicate (length inp + 1) ([])"
+  let ?bs = "replicate (length \<omega> + 1) ([])"
   have "bins (?bs[0 := ?b0]) = set (items ?b0)"
   proof -
     have "bins (?bs[0 := ?b0]) = \<Union> {set (items ((?bs[0 := ?b0]) ! k)) |k. k < length (?bs[0 := ?b0])}"
@@ -1174,53 +1174,53 @@ proof -
       by (auto simp: items_def)
     finally show ?thesis .
   qed
-  also have "... = Init\<^sub>F cfg"
+  also have "... = Init\<^sub>F \<G>"
     by (auto simp: Init\<^sub>F_def items_def rule_head_def)
   finally show ?thesis
     by (auto simp: Init\<^sub>L_def)
 qed
 
 lemma Scan\<^sub>L_sub_Scan\<^sub>F:
-  assumes "wf_bins cfg inp bs" "bins bs \<subseteq> I" "x \<in> set (items (bs ! k))" "k < length bs" "k < length inp"
+  assumes "wf_bins \<G> \<omega> bs" "bins bs \<subseteq> I" "x \<in> set (items (bs ! k))" "k < length bs" "k < length \<omega>"
   assumes "next_symbol x = Some a"
-  shows "set (items (Scan\<^sub>L k inp a x pre)) \<subseteq> Scan\<^sub>F k inp I"
+  shows "set (items (Scan\<^sub>L k \<omega> a x pre)) \<subseteq> Scan\<^sub>F k \<omega> I"
 proof standard
   fix y
-  assume *: "y \<in> set (items (Scan\<^sub>L k inp a x pre))"
+  assume *: "y \<in> set (items (Scan\<^sub>L k \<omega> a x pre))"
   have "x \<in> bin I k"
     using kth_bin_sub_bins assms(1-4) items_def wf_bin_def wf_bins_def wf_bin_items_def bin_def by fastforce
   {
-    assume #: "k < length inp" "inp!k = a"
+    assume #: "k < length \<omega>" "\<omega>!k = a"
     hence "y = inc_item x (k+1)"
       using * unfolding Scan\<^sub>L_def by (simp add: items_def)
-    hence "y \<in> Scan\<^sub>F k inp I"
+    hence "y \<in> Scan\<^sub>F k \<omega> I"
       using \<open>x \<in> bin I k\<close> # assms(6) unfolding Scan\<^sub>F_def by blast
   }
-  thus "y \<in> Scan\<^sub>F k inp I"
+  thus "y \<in> Scan\<^sub>F k \<omega> I"
     using * assms(5) unfolding Scan\<^sub>L_def by (auto simp: items_def)
 qed
 
 lemma Predict\<^sub>L_sub_Predict\<^sub>F:
-  assumes "wf_bins cfg inp bs" "bins bs \<subseteq> I" "x \<in> set (items (bs ! k))" "k < length bs"
+  assumes "wf_bins \<G> \<omega> bs" "bins bs \<subseteq> I" "x \<in> set (items (bs ! k))" "k < length bs"
   assumes "next_symbol x = Some X"
-  shows "set (items (Predict\<^sub>L k cfg X)) \<subseteq> Predict\<^sub>F k cfg I"
+  shows "set (items (Predict\<^sub>L k \<G> X)) \<subseteq> Predict\<^sub>F k \<G> I"
 proof standard
   fix y
-  assume *: "y \<in> set (items (Predict\<^sub>L k cfg X))"
+  assume *: "y \<in> set (items (Predict\<^sub>L k \<G> X))"
   have "x \<in> bin I k"
     using kth_bin_sub_bins assms(1-4) items_def wf_bin_def wf_bins_def bin_def wf_bin_items_def by fast
-  let ?rs = "filter (\<lambda>r. rule_head r = X) (\<RR> cfg)"
+  let ?rs = "filter (\<lambda>r. rule_head r = X) (\<RR> \<G>)"
   let ?xs = "map (\<lambda>r. init_item r k) ?rs"
   have "y \<in> set ?xs"
     using * unfolding Predict\<^sub>L_def items_def by simp
-  then obtain r where "y = init_item r k" "rule_head r = X" "r \<in> set (\<RR> cfg)" "next_symbol x = Some (rule_head r)"
+  then obtain r where "y = init_item r k" "rule_head r = X" "r \<in> set (\<RR> \<G>)" "next_symbol x = Some (rule_head r)"
     using assms(5) by auto
-  thus "y \<in> Predict\<^sub>F k cfg I"
+  thus "y \<in> Predict\<^sub>F k \<G> I"
     unfolding Predict\<^sub>F_def using \<open>x \<in> bin I k\<close> by blast
 qed
 
 lemma Complete\<^sub>L_sub_Complete\<^sub>F:
-  assumes "wf_bins cfg inp bs" "bins bs \<subseteq> I" "y \<in> set (items (bs ! k))" "k < length bs"
+  assumes "wf_bins \<G> \<omega> bs" "bins bs \<subseteq> I" "y \<in> set (items (bs ! k))" "k < length bs"
   assumes "next_symbol y = None"
   shows "set (items (Complete\<^sub>L k y bs red)) \<subseteq> Complete\<^sub>F k I"
 proof standard
@@ -1255,181 +1255,91 @@ proof standard
     using \<open>y \<in> bin I k\<close> assms(5) unfolding Complete\<^sub>F_def next_symbol_def by (auto split: if_splits)
 qed
 
-lemma Earley\<^sub>L_bin'_sub_Earley\<^sub>F_bin:
-  assumes "(k, cfg, inp, bs) \<in> wf_earley_input"
-  assumes "bins bs \<subseteq> I"
-  shows "bins (Earley\<^sub>L_bin' k cfg inp bs i) \<subseteq> Earley\<^sub>F_bin k cfg inp I"
-  using assms
-proof (induction i arbitrary: I rule: Earley\<^sub>L_bin'_induct[OF assms(1), case_names Base Complete\<^sub>F Scan\<^sub>F Pass Predict\<^sub>F])
-  case (Base k cfg inp bs i)
-  thus ?case
-    using Earley\<^sub>F_bin_mono by fastforce
-next
-  case (Complete\<^sub>F k cfg inp bs i x)
-  let ?bs' = "bins_upd bs k (Complete\<^sub>L k x bs i)"
-  have "x \<in> set (items (bs ! k))"
-    using Complete\<^sub>F.hyps(1,2) by force
-  hence "bins ?bs' \<subseteq> I \<union> Complete\<^sub>F k I"
-    using Complete\<^sub>L_sub_Complete\<^sub>F Complete\<^sub>F.hyps(3) Complete\<^sub>F.prems(1,2) bins_bins_upd wf_earley_input_elim by blast
-  moreover have "(k, cfg, inp, ?bs') \<in> wf_earley_input"
-    using Complete\<^sub>F.hyps Complete\<^sub>F.prems(1) wf_earley_input_Complete\<^sub>L by blast
-  ultimately have "bins (Earley\<^sub>L_bin' k cfg inp bs i) \<subseteq> Earley\<^sub>F_bin k cfg inp (I \<union> Complete\<^sub>F k I)"
-    using Complete\<^sub>F.IH Complete\<^sub>F.hyps by simp
-  also have "... \<subseteq> Earley\<^sub>F_bin k cfg inp (Earley\<^sub>F_bin k cfg inp I)"
-    using Complete\<^sub>F_Earley\<^sub>F_bin_mono Earley\<^sub>F_bin_mono Earley\<^sub>F_bin_sub_mono by (metis Un_subset_iff)
-  finally show ?case
-    using Earley\<^sub>F_bin_idem by blast
-next
-  case (Scan\<^sub>F k cfg inp bs i x a)
-  let ?bs' = "bins_upd bs (k+1) (Scan\<^sub>L k inp a x i)"
-  have "x \<in> set (items (bs ! k))"
-    using Scan\<^sub>F.hyps(1,2) by force
-  hence "bins ?bs' \<subseteq> I \<union> Scan\<^sub>F k inp I"
-    using Scan\<^sub>L_sub_Scan\<^sub>F Scan\<^sub>F.hyps(3,5) Scan\<^sub>F.prems bins_bins_upd wf_earley_input_elim
-    by (metis add_mono1 sup_mono)
-  moreover have "(k, cfg, inp, ?bs') \<in> wf_earley_input"
-    using Scan\<^sub>F.hyps Scan\<^sub>F.prems(1) wf_earley_input_Scan\<^sub>L by metis
-  ultimately have "bins (Earley\<^sub>L_bin' k cfg inp bs i) \<subseteq> Earley\<^sub>F_bin k cfg inp (I \<union> Scan\<^sub>F k inp I)"
-    using Scan\<^sub>F.IH Scan\<^sub>F.hyps by simp
-  thus ?case
-    using Scan\<^sub>F_Earley\<^sub>F_bin_mono Earley\<^sub>F_bin_mono Earley\<^sub>F_bin_sub_mono Earley\<^sub>F_bin_idem by (metis le_supI order_trans)
-next
-  case (Pass k cfg inp bs i x a)
-  thus ?case
-    by simp
-next
-  case (Predict\<^sub>F k cfg inp bs i x a)
-  let ?bs' = "bins_upd bs k (Predict\<^sub>L k cfg a)"
-  have "x \<in> set (items (bs ! k))"
-    using Predict\<^sub>F.hyps(1,2) by force
-  hence "bins ?bs' \<subseteq> I \<union> Predict\<^sub>F k cfg I"
-    using Predict\<^sub>L_sub_Predict\<^sub>F Predict\<^sub>F.hyps(3) Predict\<^sub>F.prems bins_bins_upd wf_earley_input_elim
-    by (metis sup_mono)
-  moreover have "(k, cfg, inp, ?bs') \<in> wf_earley_input"
-    using Predict\<^sub>F.hyps Predict\<^sub>F.prems(1) wf_earley_input_Predict\<^sub>L by metis
-  ultimately have "bins (Earley\<^sub>L_bin' k cfg inp bs i)  \<subseteq> Earley\<^sub>F_bin k cfg inp (I \<union> Predict\<^sub>F k cfg I)"
-    using Predict\<^sub>F.IH Predict\<^sub>F.hyps by simp
-  thus ?case
-    using Predict\<^sub>F_Earley\<^sub>F_bin_mono Earley\<^sub>F_bin_mono Earley\<^sub>F_bin_sub_mono Earley\<^sub>F_bin_idem by (metis le_supI order_trans)
-qed
-
-lemma Earley\<^sub>L_bin_sub_Earley\<^sub>F_bin:
-  assumes "(k, cfg, inp, bs) \<in> wf_earley_input"
-  assumes "bins bs \<subseteq> I"
-  shows "bins (Earley\<^sub>L_bin k cfg inp bs) \<subseteq> Earley\<^sub>F_bin k cfg inp I"
-  using assms Earley\<^sub>L_bin'_sub_Earley\<^sub>F_bin Earley\<^sub>L_bin_def by metis
-
-lemma Earley\<^sub>L_bins_sub_Earley\<^sub>F_bins:
-  assumes "k \<le> length inp" "wf_\<G> cfg"
-  shows "bins (Earley\<^sub>L_bins k cfg inp) \<subseteq> Earley\<^sub>F_bins k cfg inp"
-  using assms
-proof (induction k)
-  case 0
-  have "(k, cfg, inp, Init\<^sub>L cfg inp) \<in> wf_earley_input"
-    using assms(1) assms(2) wf_earley_input_Init\<^sub>L by blast
-  thus ?case
-    by (simp add: Init\<^sub>L_eq_Init\<^sub>F Earley\<^sub>L_bin_sub_Earley\<^sub>F_bin assms(2) wf_earley_input_Init\<^sub>L)
-next
-  case (Suc k)
-  have "(Suc k, cfg, inp, Earley\<^sub>L_bins k cfg inp) \<in> wf_earley_input"
-    by (simp add: Suc.prems(1) Suc_leD assms(2) wf_earley_input_intro)
-  thus ?case
-    by (simp add: Suc.IH Suc.prems(1) Suc_leD Earley\<^sub>L_bin_sub_Earley\<^sub>F_bin assms(2))
-qed
-
-lemma Earley\<^sub>L_sub_Earley\<^sub>F:
-  "wf_\<G> cfg \<Longrightarrow> bins (Earley\<^sub>L cfg inp) \<subseteq> Earley\<^sub>F cfg inp"
-  using Earley\<^sub>L_bins_sub_Earley\<^sub>F_bins Earley\<^sub>F_def Earley\<^sub>L_def by (metis dual_order.refl)
-
-
-
-subsection \<open>Soundness\<close>
-
 lemma sound_Scan\<^sub>L:
-  assumes "wf_bins cfg inp bs" "bins bs \<subseteq> I" "x \<in> set (items (bs!k))" "k < length bs" "k < length inp"
-  assumes "next_symbol x = Some a" "\<forall>x \<in> I. wf_item cfg inp x" "\<forall>x \<in> I. sound_item cfg inp x"
-  shows "\<forall>x \<in> set (items (Scan\<^sub>L k inp a x i)). sound_item cfg inp x"
+  assumes "wf_bins \<G> \<omega> bs" "bins bs \<subseteq> I" "x \<in> set (items (bs!k))" "k < length bs" "k < length \<omega>"
+  assumes "next_symbol x = Some a" "\<forall>x \<in> I. wf_item \<G> \<omega> x" "\<forall>x \<in> I. sound_item \<G> \<omega> x"
+  shows "\<forall>x \<in> set (items (Scan\<^sub>L k \<omega> a x i)). sound_item \<G> \<omega> x"
 proof standard
   fix y
-  assume "y \<in> set (items (Scan\<^sub>L k inp a x i))"
-  hence "y \<in> Scan\<^sub>F k inp I"
+  assume "y \<in> set (items (Scan\<^sub>L k \<omega> a x i))"
+  hence "y \<in> Scan\<^sub>F k \<omega> I"
     by (meson Scan\<^sub>L_sub_Scan\<^sub>F assms(1-6) in_mono)
-  thus "sound_item cfg inp y"
+  thus "sound_item \<G> \<omega> y"
     using sound_Scan assms(7,8) unfolding Scan\<^sub>F_def inc_item_def bin_def
     by (smt (verit, best) item.exhaust_sel mem_Collect_eq)
 qed
 
 lemma sound_Predict\<^sub>L:
-  assumes "wf_bins cfg inp bs" "bins bs \<subseteq> I" "x \<in> set (items (bs!k))" "k < length bs"
-  assumes "next_symbol x = Some X" "\<forall>x \<in> I. wf_item cfg inp x" "\<forall>x \<in> I. sound_item cfg inp x"
-  shows "\<forall>x \<in> set (items (Predict\<^sub>L k cfg X)). sound_item cfg inp x"
+  assumes "wf_bins \<G> \<omega> bs" "bins bs \<subseteq> I" "x \<in> set (items (bs!k))" "k < length bs"
+  assumes "next_symbol x = Some X" "\<forall>x \<in> I. wf_item \<G> \<omega> x" "\<forall>x \<in> I. sound_item \<G> \<omega> x"
+  shows "\<forall>x \<in> set (items (Predict\<^sub>L k \<G> X)). sound_item \<G> \<omega> x"
 proof standard
   fix y
-  assume "y \<in> set (items (Predict\<^sub>L k cfg X))"
-  hence "y \<in> Predict\<^sub>F k cfg I"
+  assume "y \<in> set (items (Predict\<^sub>L k \<G> X))"
+  hence "y \<in> Predict\<^sub>F k \<G> I"
     by (meson Predict\<^sub>L_sub_Predict\<^sub>F assms(1-5) subsetD)
-  thus "sound_item cfg inp y"
+  thus "sound_item \<G> \<omega> y"
     using sound_Predict assms(6,7) unfolding Predict\<^sub>F_def init_item_def bin_def
     by (smt (verit, del_insts) item.exhaust_sel mem_Collect_eq)
 qed
 
 lemma sound_Complete\<^sub>L:
-  assumes "wf_bins cfg inp bs" "bins bs \<subseteq> I" "y \<in> set (items (bs!k))" "k < length bs"
-  assumes "next_symbol y = None" "\<forall>x \<in> I. wf_item cfg inp x" "\<forall>x \<in> I. sound_item cfg inp x"
-  shows "\<forall>x \<in> set (items (Complete\<^sub>L k y bs i)). sound_item cfg inp x"
+  assumes "wf_bins \<G> \<omega> bs" "bins bs \<subseteq> I" "y \<in> set (items (bs!k))" "k < length bs"
+  assumes "next_symbol y = None" "\<forall>x \<in> I. wf_item \<G> \<omega> x" "\<forall>x \<in> I. sound_item \<G> \<omega> x"
+  shows "\<forall>x \<in> set (items (Complete\<^sub>L k y bs i)). sound_item \<G> \<omega> x"
 proof standard
   fix x
   assume "x \<in> set (items (Complete\<^sub>L k y bs i))"
   hence "x \<in> Complete\<^sub>F k I"
     using Complete\<^sub>L_sub_Complete\<^sub>F assms(1-5) by blast
-  thus "sound_item cfg inp x"
+  thus "sound_item \<G> \<omega> x"
     using sound_Complete assms(6,7) unfolding Complete\<^sub>F_def inc_item_def bin_def
     by (smt (verit, del_insts) item.exhaust_sel mem_Collect_eq)
 qed
 
 lemma sound_Earley\<^sub>L_bin':
-  assumes "(k, cfg, inp, bs) \<in> wf_earley_input"
-  assumes "\<forall>x \<in> bins bs. sound_item cfg inp x"
-  shows "\<forall>x \<in> bins (Earley\<^sub>L_bin' k cfg inp bs i). sound_item cfg inp x"
+  assumes "(k, \<G>, \<omega>, bs) \<in> wf_earley_input"
+  assumes "\<forall>x \<in> bins bs. sound_item \<G> \<omega> x"
+  shows "\<forall>x \<in> bins (Earley\<^sub>L_bin' k \<G> \<omega> bs i). sound_item \<G> \<omega> x"
   using assms
 proof (induction i rule: Earley\<^sub>L_bin'_induct[OF assms(1), case_names Base Complete\<^sub>F Scan\<^sub>F Pass Predict\<^sub>F])
-  case (Complete\<^sub>F k cfg inp bs i x)
+  case (Complete\<^sub>F k \<G> \<omega> bs i x)
   let ?bs' = "bins_upd bs k (Complete\<^sub>L k x bs i)"
   have "x \<in> set (items (bs ! k))"
     using Complete\<^sub>F.hyps(1,2) by force
-  hence "\<forall>x \<in> set (items (Complete\<^sub>L k x bs i)). sound_item cfg inp x"
+  hence "\<forall>x \<in> set (items (Complete\<^sub>L k x bs i)). sound_item \<G> \<omega> x"
     using sound_Complete\<^sub>L Complete\<^sub>F.hyps(3) Complete\<^sub>F.prems wf_earley_input_elim wf_bins_impl_wf_items by fastforce
-  moreover have "(k, cfg, inp, ?bs') \<in> wf_earley_input"
+  moreover have "(k, \<G>, \<omega>, ?bs') \<in> wf_earley_input"
     using Complete\<^sub>F.hyps Complete\<^sub>F.prems(1) wf_earley_input_Complete\<^sub>L by blast
-  ultimately have "\<forall>x \<in> bins (Earley\<^sub>L_bin' k cfg inp ?bs' (i + 1)). sound_item cfg inp x"
+  ultimately have "\<forall>x \<in> bins (Earley\<^sub>L_bin' k \<G> \<omega> ?bs' (i + 1)). sound_item \<G> \<omega> x"
     using Complete\<^sub>F.IH Complete\<^sub>F.prems(2) length_bins_upd bins_bins_upd wf_earley_input_elim
       Suc_eq_plus1 Un_iff le_imp_less_Suc by metis
   thus ?case
     using Complete\<^sub>F.hyps by simp
 next
-  case (Scan\<^sub>F k cfg inp bs i x a)
-  let ?bs' = "bins_upd bs (k+1) (Scan\<^sub>L k inp a x i)"
+  case (Scan\<^sub>F k \<G> \<omega> bs i x a)
+  let ?bs' = "bins_upd bs (k+1) (Scan\<^sub>L k \<omega> a x i)"
   have "x \<in> set (items (bs ! k))"
     using Scan\<^sub>F.hyps(1,2) by force
-  hence "\<forall>x \<in> set (items (Scan\<^sub>L k inp a x i)). sound_item cfg inp x"
+  hence "\<forall>x \<in> set (items (Scan\<^sub>L k \<omega> a x i)). sound_item \<G> \<omega> x"
     using sound_Scan\<^sub>L Scan\<^sub>F.hyps(3,5) Scan\<^sub>F.prems(1,2) wf_earley_input_elim wf_bins_impl_wf_items by fast
-  moreover have "(k, cfg, inp, ?bs') \<in> wf_earley_input"
+  moreover have "(k, \<G>, \<omega>, ?bs') \<in> wf_earley_input"
     using Scan\<^sub>F.hyps Scan\<^sub>F.prems(1) wf_earley_input_Scan\<^sub>L by metis
-  ultimately have "\<forall>x \<in> bins (Earley\<^sub>L_bin' k cfg inp ?bs' (i + 1)). sound_item cfg inp x"
+  ultimately have "\<forall>x \<in> bins (Earley\<^sub>L_bin' k \<G> \<omega> ?bs' (i + 1)). sound_item \<G> \<omega> x"
     using Scan\<^sub>F.IH Scan\<^sub>F.hyps(5) Scan\<^sub>F.prems(2) length_bins_upd bins_bins_upd wf_earley_input_elim
     by (metis UnE add_less_cancel_right)
   thus ?case
     using Scan\<^sub>F.hyps by simp
 next
-  case (Predict\<^sub>F k cfg inp bs i x a)
-  let ?bs' = "bins_upd bs k (Predict\<^sub>L k cfg a)"
+  case (Predict\<^sub>F k \<G> \<omega> bs i x a)
+  let ?bs' = "bins_upd bs k (Predict\<^sub>L k \<G> a)"
   have "x \<in> set (items (bs ! k))"
     using Predict\<^sub>F.hyps(1,2) by force
-  hence "\<forall>x \<in> set (items(Predict\<^sub>L k cfg a)). sound_item cfg inp x"
+  hence "\<forall>x \<in> set (items(Predict\<^sub>L k \<G> a)). sound_item \<G> \<omega> x"
     using sound_Predict\<^sub>L Predict\<^sub>F.hyps(3) Predict\<^sub>F.prems wf_earley_input_elim wf_bins_impl_wf_items by fast
-  moreover have "(k, cfg, inp, ?bs') \<in> wf_earley_input"
+  moreover have "(k, \<G>, \<omega>, ?bs') \<in> wf_earley_input"
     using Predict\<^sub>F.hyps Predict\<^sub>F.prems(1) wf_earley_input_Predict\<^sub>L by metis
-  ultimately have "\<forall>x \<in> bins (Earley\<^sub>L_bin' k cfg inp ?bs' (i + 1)). sound_item cfg inp x"
+  ultimately have "\<forall>x \<in> bins (Earley\<^sub>L_bin' k \<G> \<omega> ?bs' (i + 1)). sound_item \<G> \<omega> x"
     using Predict\<^sub>F.IH Predict\<^sub>F.prems(2) length_bins_upd bins_bins_upd wf_earley_input_elim
     by (metis Suc_eq_plus1 UnE)
   thus ?case
@@ -1437,30 +1347,121 @@ next
 qed simp_all
 
 lemma sound_Earley\<^sub>L_bin:
-  assumes "(k, cfg, inp, bs) \<in> wf_earley_input"
-  assumes "\<forall>x \<in> bins bs. sound_item cfg inp x"
-  shows "\<forall>x \<in> bins (Earley\<^sub>L_bin k cfg inp bs). sound_item cfg inp x"
+  assumes "(k, \<G>, \<omega>, bs) \<in> wf_earley_input"
+  assumes "\<forall>x \<in> bins bs. sound_item \<G> \<omega> x"
+  shows "\<forall>x \<in> bins (Earley\<^sub>L_bin k \<G> \<omega> bs). sound_item \<G> \<omega> x"
   using sound_Earley\<^sub>L_bin' assms Earley\<^sub>L_bin_def by metis
 
+lemma Earley\<^sub>L_bin'_sub_Earley\<^sub>F_bin:
+  assumes "(k, \<G>, \<omega>, bs) \<in> wf_earley_input"
+  assumes "bins bs \<subseteq> I"
+  shows "bins (Earley\<^sub>L_bin' k \<G> \<omega> bs i) \<subseteq> Earley\<^sub>F_bin k \<G> \<omega> I"
+  using assms
+proof (induction i arbitrary: I rule: Earley\<^sub>L_bin'_induct[OF assms(1), case_names Base Complete\<^sub>F Scan\<^sub>F Pass Predict\<^sub>F])
+  case (Base k \<G> \<omega> bs i)
+  thus ?case
+    using Earley\<^sub>F_bin_mono by fastforce
+next
+  case (Complete\<^sub>F k \<G> \<omega> bs i x)
+  let ?bs' = "bins_upd bs k (Complete\<^sub>L k x bs i)"
+  have "x \<in> set (items (bs ! k))"
+    using Complete\<^sub>F.hyps(1,2) by force
+  hence "bins ?bs' \<subseteq> I \<union> Complete\<^sub>F k I"
+    using Complete\<^sub>L_sub_Complete\<^sub>F Complete\<^sub>F.hyps(3) Complete\<^sub>F.prems(1,2) bins_bins_upd wf_earley_input_elim by blast
+  moreover have "(k, \<G>, \<omega>, ?bs') \<in> wf_earley_input"
+    using Complete\<^sub>F.hyps Complete\<^sub>F.prems(1) wf_earley_input_Complete\<^sub>L by blast
+  ultimately have "bins (Earley\<^sub>L_bin' k \<G> \<omega> bs i) \<subseteq> Earley\<^sub>F_bin k \<G> \<omega> (I \<union> Complete\<^sub>F k I)"
+    using Complete\<^sub>F.IH Complete\<^sub>F.hyps by simp
+  also have "... \<subseteq> Earley\<^sub>F_bin k \<G> \<omega> (Earley\<^sub>F_bin k \<G> \<omega> I)"
+    using Complete\<^sub>F_Earley\<^sub>F_bin_mono Earley\<^sub>F_bin_mono Earley\<^sub>F_bin_sub_mono by (metis Un_subset_iff)
+  finally show ?case
+    using Earley\<^sub>F_bin_idem by blast
+next
+  case (Scan\<^sub>F k \<G> \<omega> bs i x a)
+  let ?bs' = "bins_upd bs (k+1) (Scan\<^sub>L k \<omega> a x i)"
+  have "x \<in> set (items (bs ! k))"
+    using Scan\<^sub>F.hyps(1,2) by force
+  hence "bins ?bs' \<subseteq> I \<union> Scan\<^sub>F k \<omega> I"
+    using Scan\<^sub>L_sub_Scan\<^sub>F Scan\<^sub>F.hyps(3,5) Scan\<^sub>F.prems bins_bins_upd wf_earley_input_elim
+    by (metis add_mono1 sup_mono)
+  moreover have "(k, \<G>, \<omega>, ?bs') \<in> wf_earley_input"
+    using Scan\<^sub>F.hyps Scan\<^sub>F.prems(1) wf_earley_input_Scan\<^sub>L by metis
+  ultimately have "bins (Earley\<^sub>L_bin' k \<G> \<omega> bs i) \<subseteq> Earley\<^sub>F_bin k \<G> \<omega> (I \<union> Scan\<^sub>F k \<omega> I)"
+    using Scan\<^sub>F.IH Scan\<^sub>F.hyps by simp
+  thus ?case
+    using Scan\<^sub>F_Earley\<^sub>F_bin_mono Earley\<^sub>F_bin_mono Earley\<^sub>F_bin_sub_mono Earley\<^sub>F_bin_idem by (metis le_supI order_trans)
+next
+  case (Pass k \<G> \<omega> bs i x a)
+  thus ?case
+    by simp
+next
+  case (Predict\<^sub>F k \<G> \<omega> bs i x a)
+  let ?bs' = "bins_upd bs k (Predict\<^sub>L k \<G> a)"
+  have "x \<in> set (items (bs ! k))"
+    using Predict\<^sub>F.hyps(1,2) by force
+  hence "bins ?bs' \<subseteq> I \<union> Predict\<^sub>F k \<G> I"
+    using Predict\<^sub>L_sub_Predict\<^sub>F Predict\<^sub>F.hyps(3) Predict\<^sub>F.prems bins_bins_upd wf_earley_input_elim
+    by (metis sup_mono)
+  moreover have "(k, \<G>, \<omega>, ?bs') \<in> wf_earley_input"
+    using Predict\<^sub>F.hyps Predict\<^sub>F.prems(1) wf_earley_input_Predict\<^sub>L by metis
+  ultimately have "bins (Earley\<^sub>L_bin' k \<G> \<omega> bs i)  \<subseteq> Earley\<^sub>F_bin k \<G> \<omega> (I \<union> Predict\<^sub>F k \<G> I)"
+    using Predict\<^sub>F.IH Predict\<^sub>F.hyps by simp
+  thus ?case
+    using Predict\<^sub>F_Earley\<^sub>F_bin_mono Earley\<^sub>F_bin_mono Earley\<^sub>F_bin_sub_mono Earley\<^sub>F_bin_idem by (metis le_supI order_trans)
+qed
 
-subsection \<open>Set to list\<close>
+lemma Earley\<^sub>L_bin_sub_Earley\<^sub>F_bin:
+  assumes "(k, \<G>, \<omega>, bs) \<in> wf_earley_input"
+  assumes "bins bs \<subseteq> I"
+  shows "bins (Earley\<^sub>L_bin k \<G> \<omega> bs) \<subseteq> Earley\<^sub>F_bin k \<G> \<omega> I"
+  using assms Earley\<^sub>L_bin'_sub_Earley\<^sub>F_bin Earley\<^sub>L_bin_def by metis
+
+lemma Earley\<^sub>L_bins_sub_Earley\<^sub>F_bins:
+  assumes "k \<le> length \<omega>" "wf_\<G> \<G>"
+  shows "bins (Earley\<^sub>L_bins k \<G> \<omega>) \<subseteq> Earley\<^sub>F_bins k \<G> \<omega>"
+  using assms
+proof (induction k)
+  case 0
+  have "(k, \<G>, \<omega>, Init\<^sub>L \<G> \<omega>) \<in> wf_earley_input"
+    using assms(1) assms(2) wf_earley_input_Init\<^sub>L by blast
+  thus ?case
+    by (simp add: Init\<^sub>L_eq_Init\<^sub>F Earley\<^sub>L_bin_sub_Earley\<^sub>F_bin assms(2) wf_earley_input_Init\<^sub>L)
+next
+  case (Suc k)
+  have "(Suc k, \<G>, \<omega>, Earley\<^sub>L_bins k \<G> \<omega>) \<in> wf_earley_input"
+    by (simp add: Suc.prems(1) Suc_leD assms(2) wf_earley_input_intro)
+  thus ?case
+    by (simp add: Suc.IH Suc.prems(1) Suc_leD Earley\<^sub>L_bin_sub_Earley\<^sub>F_bin assms(2))
+qed
+
+lemma Earley\<^sub>L_sub_Earley\<^sub>F:
+  "wf_\<G> \<G> \<Longrightarrow> bins (Earley\<^sub>L \<G> \<omega>) \<subseteq> Earley\<^sub>F \<G> \<omega>"
+  using Earley\<^sub>L_bins_sub_Earley\<^sub>F_bins Earley\<^sub>F_def Earley\<^sub>L_def by (metis dual_order.refl)
+
+theorem soundness_Earley\<^sub>L:
+  assumes "wf_\<G> \<G>" "recognizing (bins (Earley\<^sub>L \<G> \<omega>)) \<G> \<omega>"
+  shows "derives \<G> [\<SS> \<G>] \<omega>"
+  using assms Earley\<^sub>L_sub_Earley\<^sub>F recognizing_def soundness_Earley\<^sub>F by (meson subsetD)
+
+
+subsection \<open>Completeness\<close>
 
 lemma bin_bins_upto_bins_eq:
-  assumes "wf_bins cfg inp bs" "k < length bs" "i \<ge> length (items (bs ! k))" "l \<le> k"
+  assumes "wf_bins \<G> \<omega> bs" "k < length bs" "i \<ge> length (items (bs ! k))" "l \<le> k"
   shows "bin (bins_upto bs k i) l = bin (bins bs) l"
   unfolding bins_upto_def bins_def bin_def using assms nat_less_le
   apply (auto simp: nth_list_update bin_upto_eq_set_items wf_bins_kth_bin items_def)
-  apply (metis imageI nle_le order_trans, fast)
+   apply (metis imageI nle_le order_trans, fast)
   done
 
 lemma impossible_complete_item:
-  assumes "wf_\<G> cfg" "wf_item cfg inp x" "sound_item cfg inp x"
-  assumes "is_complete x"  "item_origin x = k" "item_end x = k" "nonempty_derives cfg"
+  assumes "wf_\<G> \<G>" "wf_item \<G> \<omega> x" "sound_item \<G> \<omega> x"
+  assumes "is_complete x"  "item_origin x = k" "item_end x = k" "nonempty_derives \<G>"
   shows False
 proof -
-  have "derives cfg [item_rule_head x] []"
+  have "derives \<G> [item_rule_head x] []"
     using assms(3-6) by (simp add: slice_empty is_complete_def sound_item_def item_\<beta>_def )
-  moreover have "is_nonterminal cfg (item_rule_head x)"
+  moreover have "is_nonterminal \<G> (item_rule_head x)"
     using assms(1,2) unfolding wf_item_def item_rule_head_def rule_head_def
     by (metis prod.collapse rule_nonterminal_type)
   ultimately show ?thesis
@@ -1468,7 +1469,7 @@ proof -
 qed
 
 lemma Complete\<^sub>F_Un_eq_terminal:
-  assumes "next_symbol z = Some a" "is_terminal cfg a" "\<forall>x \<in> I. wf_item cfg inp x" "wf_item cfg inp z" "wf_\<G> cfg"
+  assumes "next_symbol z = Some a" "is_terminal \<G> a" "\<forall>x \<in> I. wf_item \<G> \<omega> x" "wf_item \<G> \<omega> z" "wf_\<G> \<G>"
   shows "Complete\<^sub>F k (I \<union> {z}) = Complete\<^sub>F k I"
 proof (rule ccontr)
   assume "Complete\<^sub>F k (I \<union> {z}) \<noteq> Complete\<^sub>F k I"
@@ -1482,7 +1483,7 @@ proof (rule ccontr)
   show False
   proof (cases "x = z")
     case True
-    have "is_nonterminal cfg (item_rule_head y)"
+    have "is_nonterminal \<G> (item_rule_head y)"
       using *(5,6) assms(1,3-5)
       apply (auto simp: wf_item_def bin_def item_rule_head_def rule_head_def next_symbol_def)
       by (metis prod.exhaust_sel rule_nonterminal_type)
@@ -1496,8 +1497,8 @@ proof (rule ccontr)
 qed
 
 lemma Complete\<^sub>F_Un_eq_nonterminal:
-  assumes "wf_\<G> cfg" "\<forall>x \<in> I. wf_item cfg inp x" "\<forall>x \<in> I. sound_item cfg inp x"
-  assumes "nonempty_derives cfg" "wf_item cfg inp z"
+  assumes "wf_\<G> \<G>" "\<forall>x \<in> I. wf_item \<G> \<omega> x" "\<forall>x \<in> I. sound_item \<G> \<omega> x"
+  assumes "nonempty_derives \<G>" "wf_item \<G> \<omega> z"
   assumes "item_end z = k" "next_symbol z \<noteq> None"
   shows "Complete\<^sub>F k (I \<union> {z}) = Complete\<^sub>F k I"
 proof (rule ccontr)
@@ -1518,9 +1519,9 @@ proof (rule ccontr)
       using *(4) A bin_def assms(6) by (metis (mono_tags, lifting) mem_Collect_eq)
     moreover have "item_end y = k"
       using *(5) bin_def by blast
-    moreover have "sound_item cfg inp y"
+    moreover have "sound_item \<G> \<omega> y"
       using *(5,6) assms(3,7) by (auto simp: bin_def next_symbol_def sound_item_def)
-    moreover have "wf_item cfg inp y"
+    moreover have "wf_item \<G> \<omega> y"
       using *(5) assms(2,5) wf_item_def by (auto simp: bin_def)
     ultimately show ?thesis
       using impossible_complete_item *(6) assms(1,4) by blast
@@ -1532,23 +1533,23 @@ proof (rule ccontr)
 qed
 
 lemma wf_item_in_kth_bin:
-  "wf_bins cfg inp bs \<Longrightarrow> x \<in> bins bs \<Longrightarrow> item_end x = k \<Longrightarrow> x \<in> set (items (bs ! k))"
+  "wf_bins \<G> \<omega> bs \<Longrightarrow> x \<in> bins bs \<Longrightarrow> item_end x = k \<Longrightarrow> x \<in> set (items (bs ! k))"
   using bins_bin_exists wf_bins_kth_bin wf_bins_def by blast
 
 lemma Complete\<^sub>F_bins_upto_eq_bins:
-  assumes "wf_bins cfg inp bs" "k < length bs" "i \<ge> length (items (bs ! k))"
+  assumes "wf_bins \<G> \<omega> bs" "k < length bs" "i \<ge> length (items (bs ! k))"
   shows "Complete\<^sub>F k (bins_upto bs k i) = Complete\<^sub>F k (bins bs)"
 proof -
   have "\<And>l. l \<le> k \<Longrightarrow> bin (bins_upto bs k i) l = bin (bins bs) l"
     using bin_bins_upto_bins_eq[OF assms] by blast
-  moreover have "\<forall>x \<in> bins bs. wf_item cfg inp x"
+  moreover have "\<forall>x \<in> bins bs. wf_item \<G> \<omega> x"
     using assms(1) wf_bins_impl_wf_items by metis
   ultimately show ?thesis
     unfolding Complete\<^sub>F_def bin_def wf_item_def wf_item_def by auto
 qed
 
 lemma Complete\<^sub>F_sub_bins_Un_Complete\<^sub>L:
-  assumes "Complete\<^sub>F k I \<subseteq> bins bs" "I \<subseteq> bins bs" "is_complete z" "wf_bins cfg inp bs" "wf_item cfg inp z"
+  assumes "Complete\<^sub>F k I \<subseteq> bins bs" "I \<subseteq> bins bs" "is_complete z" "wf_bins \<G> \<omega> bs" "wf_item \<G> \<omega> z"
   shows "Complete\<^sub>F k (I \<union> {z}) \<subseteq> bins bs \<union> set (items (Complete\<^sub>L k z bs red))"
 proof standard
   fix w
@@ -1588,7 +1589,7 @@ lemma Complete\<^sub>L_eq_item_origin:
   by (auto simp: Complete\<^sub>L_def)
 
 lemma kth_bin_bins_upto_empty:
-  assumes "wf_bins cfg inp bs" "k < length bs"
+  assumes "wf_bins \<G> \<omega> bs" "k < length bs"
   shows "bin (bins_upto bs k 0) k = {}"
 proof -
   {
@@ -1606,93 +1607,94 @@ proof -
 qed
 
 lemma Earley\<^sub>L_bin'_mono:
-  assumes "(k, cfg, inp, bs) \<in> wf_earley_input"
-  shows "bins bs \<subseteq> bins (Earley\<^sub>L_bin' k cfg inp bs i)"
+  assumes "(k, \<G>, \<omega>, bs) \<in> wf_earley_input"
+  shows "bins bs \<subseteq> bins (Earley\<^sub>L_bin' k \<G> \<omega> bs i)"
   using assms
 proof (induction i rule: Earley\<^sub>L_bin'_induct[OF assms(1), case_names Base Complete\<^sub>F Scan\<^sub>F Pass Predict\<^sub>F])
-  case (Complete\<^sub>F k cfg inp bs i x)
+  case (Complete\<^sub>F k \<G> \<omega> bs i x)
   let ?bs' = "bins_upd bs k (Complete\<^sub>L k x bs i)"
-  have wf: "(k, cfg, inp, ?bs') \<in> wf_earley_input"
+  have wf: "(k, \<G>, \<omega>, ?bs') \<in> wf_earley_input"
     using Complete\<^sub>F.hyps Complete\<^sub>F.prems(1) wf_earley_input_Complete\<^sub>L by blast
   hence "bins bs \<subseteq> bins ?bs'"
     using length_bins_upd bins_bins_upd wf_earley_input_elim by (metis Un_upper1)
-  also have "... \<subseteq> bins (Earley\<^sub>L_bin' k cfg inp ?bs' (i + 1))"
+  also have "... \<subseteq> bins (Earley\<^sub>L_bin' k \<G> \<omega> ?bs' (i + 1))"
     using wf Complete\<^sub>F.IH by blast
   finally show ?case
     using Complete\<^sub>F.hyps by simp
 next
-  case (Scan\<^sub>F k cfg inp bs i x a)
-  let ?bs' = "bins_upd bs (k+1) (Scan\<^sub>L k inp a x i)"
-  have wf: "(k, cfg, inp, ?bs') \<in> wf_earley_input"
+  case (Scan\<^sub>F k \<G> \<omega> bs i x a)
+  let ?bs' = "bins_upd bs (k+1) (Scan\<^sub>L k \<omega> a x i)"
+  have wf: "(k, \<G>, \<omega>, ?bs') \<in> wf_earley_input"
     using Scan\<^sub>F.hyps Scan\<^sub>F.prems(1) wf_earley_input_Scan\<^sub>L by metis
   hence "bins bs \<subseteq> bins ?bs'"
     using Scan\<^sub>F.hyps(5) length_bins_upd bins_bins_upd wf_earley_input_elim
     by (metis add_mono1 sup_ge1)
-  also have "... \<subseteq> bins (Earley\<^sub>L_bin' k cfg inp ?bs' (i + 1))"
+  also have "... \<subseteq> bins (Earley\<^sub>L_bin' k \<G> \<omega> ?bs' (i + 1))"
     using wf Scan\<^sub>F.IH by blast
   finally show ?case
     using Scan\<^sub>F.hyps by simp
 next
-  case (Predict\<^sub>F k cfg inp bs i x a)
-  let ?bs' = "bins_upd bs k (Predict\<^sub>L k cfg a)"
-  have wf: "(k, cfg, inp, ?bs') \<in> wf_earley_input"
+  case (Predict\<^sub>F k \<G> \<omega> bs i x a)
+  let ?bs' = "bins_upd bs k (Predict\<^sub>L k \<G> a)"
+  have wf: "(k, \<G>, \<omega>, ?bs') \<in> wf_earley_input"
     using Predict\<^sub>F.hyps Predict\<^sub>F.prems(1) wf_earley_input_Predict\<^sub>L by metis
   hence "bins bs \<subseteq> bins ?bs'"
     using length_bins_upd bins_bins_upd wf_earley_input_elim by (metis sup_ge1)
-  also have "... \<subseteq> bins (Earley\<^sub>L_bin' k cfg inp ?bs' (i + 1))"
+  also have "... \<subseteq> bins (Earley\<^sub>L_bin' k \<G> \<omega> ?bs' (i + 1))"
     using wf Predict\<^sub>F.IH by blast
   finally show ?case
     using Predict\<^sub>F.hyps by simp
 qed simp_all
 
 lemma Earley\<^sub>F_bin_step_sub_Earley\<^sub>L_bin':
-  assumes "(k, cfg, inp, bs) \<in> wf_earley_input"
-  assumes "Earley\<^sub>F_bin_step k cfg inp (bins_upto bs k i) \<subseteq> bins bs"
-  assumes "\<forall>x \<in> bins bs. sound_item cfg inp x" "is_word cfg inp" "nonempty_derives cfg"
-  shows "Earley\<^sub>F_bin_step k cfg inp (bins bs) \<subseteq> bins (Earley\<^sub>L_bin' k cfg inp bs i)"
+  assumes "(k, \<G>, \<omega>, bs) \<in> wf_earley_input"
+  assumes "Earley\<^sub>F_bin_step k \<G> \<omega> (bins_upto bs k i) \<subseteq> bins bs"
+  assumes "\<forall>x \<in> bins bs. sound_item \<G> \<omega> x" "is_word \<G> \<omega>" "nonempty_derives \<G>"
+  shows "Earley\<^sub>F_bin_step k \<G> \<omega> (bins bs) \<subseteq> bins (Earley\<^sub>L_bin' k \<G> \<omega> bs i)"
   using assms
 proof (induction i rule: Earley\<^sub>L_bin'_induct[OF assms(1), case_names Base Complete\<^sub>F Scan\<^sub>F Pass Predict\<^sub>F])
-  case (Base k cfg inp bs i)
+  case (Base k \<G> \<omega> bs i)
   have "bin (bins bs) k = bin (bins_upto bs k i) k"
     using Base.hyps Base.prems(1) bin_bins_upto_bins_eq wf_earley_input_elim by blast
   thus ?case
     using Scan\<^sub>F_bin_absorb Predict\<^sub>F_bin_absorb Complete\<^sub>F_bins_upto_eq_bins wf_earley_input_elim
-      Base.hyps Base.prems(1,2,3,5) Earley\<^sub>F_bin_step_def Complete\<^sub>F_Earley\<^sub>F_bin_step_mono Predict\<^sub>F_Earley\<^sub>F_bin_step_mono Scan\<^sub>F_Earley\<^sub>F_bin_step_mono Earley\<^sub>L_bin'_mono
+      Base.hyps Base.prems(1,2,3,5) Earley\<^sub>F_bin_step_def Complete\<^sub>F_Earley\<^sub>F_bin_step_mono
+      Predict\<^sub>F_Earley\<^sub>F_bin_step_mono Scan\<^sub>F_Earley\<^sub>F_bin_step_mono Earley\<^sub>L_bin'_mono
     by (metis (no_types, lifting) Un_assoc sup.orderE)
 next
-  case (Complete\<^sub>F k cfg inp bs i x)
+  case (Complete\<^sub>F k \<G> \<omega> bs i x)
   let ?bs' = "bins_upd bs k (Complete\<^sub>L k x bs i)"
   have x: "x \<in> set (items (bs ! k))"
     using Complete\<^sub>F.hyps(1,2) by auto
-  have wf: "(k, cfg, inp, ?bs') \<in> wf_earley_input"
+  have wf: "(k, \<G>, \<omega>, ?bs') \<in> wf_earley_input"
     using Complete\<^sub>F.hyps Complete\<^sub>F.prems(1) wf_earley_input_Complete\<^sub>L by blast
-  hence sound: "\<forall>x \<in> set (items (Complete\<^sub>L k x bs i)). sound_item cfg inp x"
+  hence sound: "\<forall>x \<in> set (items (Complete\<^sub>L k x bs i)). sound_item \<G> \<omega> x"
     using sound_Complete\<^sub>L Complete\<^sub>F.hyps(3) Complete\<^sub>F.prems wf_earley_input_elim wf_bins_impl_wf_items x
     by (metis dual_order.refl)
-  have "Scan\<^sub>F k inp (bins_upto ?bs' k (i + 1)) \<subseteq> bins ?bs'"
+  have "Scan\<^sub>F k \<omega> (bins_upto ?bs' k (i + 1)) \<subseteq> bins ?bs'"
   proof -
-    have "Scan\<^sub>F k inp (bins_upto ?bs' k (i + 1)) = Scan\<^sub>F k inp (bins_upto ?bs' k i \<union> {items (?bs' ! k) ! i})"
+    have "Scan\<^sub>F k \<omega> (bins_upto ?bs' k (i + 1)) = Scan\<^sub>F k \<omega> (bins_upto ?bs' k i \<union> {items (?bs' ! k) ! i})"
       using Complete\<^sub>F.hyps(1) bins_upto_Suc_Un length_nth_bin_bins_upd items_def
       by (metis length_map linorder_not_less sup.boundedE sup.order_iff)
-    also have "... = Scan\<^sub>F k inp (bins_upto bs k i \<union> {x})"
+    also have "... = Scan\<^sub>F k \<omega> (bins_upto bs k i \<union> {x})"
       using Complete\<^sub>F.hyps(1,2) Complete\<^sub>F.prems(1) items_nth_idem_bins_upd bins_upto_kth_nth_idem wf_earley_input_elim
       by (metis dual_order.refl items_def length_map not_le_imp_less)
-    also have "... \<subseteq> bins bs \<union> Scan\<^sub>F k inp {x}"
+    also have "... \<subseteq> bins bs \<union> Scan\<^sub>F k \<omega> {x}"
       using Complete\<^sub>F.prems(2,3) Scan\<^sub>F_Un Scan\<^sub>F_Earley\<^sub>F_bin_step_mono by fastforce
     also have "... = bins bs"
       using Complete\<^sub>F.hyps(3) by (auto simp: Scan\<^sub>F_def bin_def)
     finally show ?thesis
       using Complete\<^sub>F.prems(1) wf_earley_input_elim bins_bins_upd by blast
   qed
-  moreover have "Predict\<^sub>F k cfg (bins_upto ?bs' k (i + 1)) \<subseteq> bins ?bs'"
+  moreover have "Predict\<^sub>F k \<G> (bins_upto ?bs' k (i + 1)) \<subseteq> bins ?bs'"
   proof -
-    have "Predict\<^sub>F k cfg (bins_upto ?bs' k (i + 1)) = Predict\<^sub>F k cfg (bins_upto ?bs' k i \<union> {items (?bs' ! k) ! i})"
+    have "Predict\<^sub>F k \<G> (bins_upto ?bs' k (i + 1)) = Predict\<^sub>F k \<G> (bins_upto ?bs' k i \<union> {items (?bs' ! k) ! i})"
       using Complete\<^sub>F.hyps(1) bins_upto_Suc_Un length_nth_bin_bins_upd
       by (metis dual_order.strict_trans1 items_def length_map not_le_imp_less)
-    also have "... = Predict\<^sub>F k cfg (bins_upto bs k i \<union> {x})"
+    also have "... = Predict\<^sub>F k \<G> (bins_upto bs k i \<union> {x})"
       using Complete\<^sub>F.hyps(1,2) Complete\<^sub>F.prems(1) items_nth_idem_bins_upd bins_upto_kth_nth_idem wf_earley_input_elim
       by (metis dual_order.refl items_def length_map not_le_imp_less)
-    also have "... \<subseteq> bins bs \<union> Predict\<^sub>F k cfg {x}"
+    also have "... \<subseteq> bins bs \<union> Predict\<^sub>F k \<G> {x}"
       using Complete\<^sub>F.prems(2,3) Predict\<^sub>F_Un Predict\<^sub>F_Earley\<^sub>F_bin_step_mono by blast
     also have "... = bins bs"
       using Complete\<^sub>F.hyps(3) by (auto simp: Predict\<^sub>F_def bin_def)
@@ -1714,7 +1716,7 @@ next
     finally show ?thesis
       using Complete\<^sub>F.prems(1) wf_earley_input_elim bins_bins_upd by blast
   qed
-  ultimately have "Earley\<^sub>F_bin_step k cfg inp (bins ?bs') \<subseteq> bins (Earley\<^sub>L_bin' k cfg inp ?bs' (i+1))"
+  ultimately have "Earley\<^sub>F_bin_step k \<G> \<omega> (bins ?bs') \<subseteq> bins (Earley\<^sub>L_bin' k \<G> \<omega> ?bs' (i+1))"
     using Complete\<^sub>F.IH Complete\<^sub>F.prems sound wf Earley\<^sub>F_bin_step_def bins_upto_sub_bins
       wf_earley_input_elim bins_bins_upd
     by (metis UnE sup.boundedI)
@@ -1722,44 +1724,44 @@ next
     using Complete\<^sub>F.hyps Complete\<^sub>F.prems(1) Earley\<^sub>L_bin'_simps(2) Earley\<^sub>F_bin_step_sub_mono bins_bins_upd wf_earley_input_elim
     by (smt (verit, best) sup.coboundedI2 sup.orderE sup_ge1)
 next
-  case (Scan\<^sub>F k cfg inp bs i x a)
-  let ?bs' = "bins_upd bs (k+1) (Scan\<^sub>L k inp a x i)"
+  case (Scan\<^sub>F k \<G> \<omega> bs i x a)
+  let ?bs' = "bins_upd bs (k+1) (Scan\<^sub>L k \<omega> a x i)"
   have x: "x \<in> set (items (bs ! k))"
     using Scan\<^sub>F.hyps(1,2) by auto
-  hence sound: "\<forall>x \<in> set (items (Scan\<^sub>L k inp a x i)). sound_item cfg inp x"
+  hence sound: "\<forall>x \<in> set (items (Scan\<^sub>L k \<omega> a x i)). sound_item \<G> \<omega> x"
     using sound_Scan\<^sub>L Scan\<^sub>F.hyps(3,5) Scan\<^sub>F.prems(1,2,3) wf_earley_input_elim wf_bins_impl_wf_items x
     by (metis dual_order.refl)
-  have wf: "(k, cfg, inp, ?bs') \<in> wf_earley_input"
+  have wf: "(k, \<G>, \<omega>, ?bs') \<in> wf_earley_input"
     using Scan\<^sub>F.hyps Scan\<^sub>F.prems(1) wf_earley_input_Scan\<^sub>L by metis
-  have "Scan\<^sub>F k inp (bins_upto ?bs' k (i + 1)) \<subseteq> bins ?bs'"
+  have "Scan\<^sub>F k \<omega> (bins_upto ?bs' k (i + 1)) \<subseteq> bins ?bs'"
   proof -
-    have "Scan\<^sub>F k inp (bins_upto ?bs' k (i + 1)) = Scan\<^sub>F k inp (bins_upto ?bs' k i \<union> {items (?bs' ! k) ! i})"
+    have "Scan\<^sub>F k \<omega> (bins_upto ?bs' k (i + 1)) = Scan\<^sub>F k \<omega> (bins_upto ?bs' k i \<union> {items (?bs' ! k) ! i})"
       using bins_upto_Suc_Un Scan\<^sub>F.hyps(1) nth_idem_bins_upd
       by (metis Suc_eq_plus1 items_def length_map lessI less_not_refl not_le_imp_less)
-    also have "... = Scan\<^sub>F k inp (bins_upto bs k i \<union> {x})"
+    also have "... = Scan\<^sub>F k \<omega> (bins_upto bs k i \<union> {x})"
       using Scan\<^sub>F.hyps(1,2,5) Scan\<^sub>F.prems(1,2) nth_idem_bins_upd bins_upto_kth_nth_idem wf_earley_input_elim
       by (metis add_mono_thms_linordered_field(1) items_def length_map less_add_one linorder_le_less_linear not_add_less1)
-    also have "... \<subseteq> bins bs \<union> Scan\<^sub>F k inp {x}"
+    also have "... \<subseteq> bins bs \<union> Scan\<^sub>F k \<omega> {x}"
       using Scan\<^sub>F.prems(2,3) Scan\<^sub>F_Un Scan\<^sub>F_Earley\<^sub>F_bin_step_mono by fastforce
-    finally have *: "Scan\<^sub>F k inp (bins_upto ?bs' k (i + 1)) \<subseteq> bins bs \<union> Scan\<^sub>F k inp {x}" .
+    finally have *: "Scan\<^sub>F k \<omega> (bins_upto ?bs' k (i + 1)) \<subseteq> bins bs \<union> Scan\<^sub>F k \<omega> {x}" .
     show ?thesis
     proof cases
-      assume a1: "inp!k = a"
-      hence "Scan\<^sub>F k inp {x} = {inc_item x (k+1)}"
+      assume a1: "\<omega>!k = a"
+      hence "Scan\<^sub>F k \<omega> {x} = {inc_item x (k+1)}"
         using Scan\<^sub>F.hyps(1-3,5) Scan\<^sub>F.prems(1,2) wf_earley_input_elim apply (auto simp: Scan\<^sub>F_def bin_def)
         using wf_bins_kth_bin x by blast
-      hence "Scan\<^sub>F k inp (bins_upto ?bs' k (i + 1)) \<subseteq> bins bs \<union> {inc_item x (k+1)}"
+      hence "Scan\<^sub>F k \<omega> (bins_upto ?bs' k (i + 1)) \<subseteq> bins bs \<union> {inc_item x (k+1)}"
         using * by blast
-      also have "... = bins bs \<union> set (items (Scan\<^sub>L k inp a x i))"
+      also have "... = bins bs \<union> set (items (Scan\<^sub>L k \<omega> a x i))"
         using a1 Scan\<^sub>F.hyps(5) by (auto simp: Scan\<^sub>L_def items_def)
       also have "... = bins ?bs'"
         using Scan\<^sub>F.hyps(5) Scan\<^sub>F.prems(1) wf_earley_input_elim bins_bins_upd by (metis add_mono1)
       finally show ?thesis .
     next
-      assume a1: "\<not> inp!k = a"
-      hence "Scan\<^sub>F k inp {x} = {}"
+      assume a1: "\<not> \<omega>!k = a"
+      hence "Scan\<^sub>F k \<omega> {x} = {}"
         using Scan\<^sub>F.hyps(3) by (auto simp: Scan\<^sub>F_def bin_def)
-      hence "Scan\<^sub>F k inp (bins_upto ?bs' k (i + 1)) \<subseteq> bins bs"
+      hence "Scan\<^sub>F k \<omega> (bins_upto ?bs' k (i + 1)) \<subseteq> bins bs"
         using * by blast
       also have "... \<subseteq> bins ?bs'"
         using Scan\<^sub>F.hyps(5) Scan\<^sub>F.prems(1) wf_earley_input_elim bins_bins_upd
@@ -1767,15 +1769,15 @@ next
       finally show ?thesis .
     qed
   qed
-  moreover have "Predict\<^sub>F k cfg (bins_upto ?bs' k (i + 1)) \<subseteq> bins ?bs'"
+  moreover have "Predict\<^sub>F k \<G> (bins_upto ?bs' k (i + 1)) \<subseteq> bins ?bs'"
   proof -
-    have "Predict\<^sub>F k cfg (bins_upto ?bs' k (i + 1)) = Predict\<^sub>F k cfg (bins_upto ?bs' k i \<union> {items (?bs' ! k) ! i})"
+    have "Predict\<^sub>F k \<G> (bins_upto ?bs' k (i + 1)) = Predict\<^sub>F k \<G> (bins_upto ?bs' k i \<union> {items (?bs' ! k) ! i})"
       using bins_upto_Suc_Un Scan\<^sub>F.hyps(1) nth_idem_bins_upd
       by (metis Suc_eq_plus1 dual_order.refl items_def length_map lessI linorder_not_less)
-    also have "... = Predict\<^sub>F k cfg (bins_upto bs k i \<union> {x})"
+    also have "... = Predict\<^sub>F k \<G> (bins_upto bs k i \<union> {x})"
       using Scan\<^sub>F.hyps(1,2,5) Scan\<^sub>F.prems(1,2) nth_idem_bins_upd bins_upto_kth_nth_idem wf_earley_input_elim
       by (metis add_strict_right_mono items_def le_add1 length_map less_add_one linorder_not_le)
-    also have "... \<subseteq> bins bs \<union> Predict\<^sub>F k cfg {x}"
+    also have "... \<subseteq> bins bs \<union> Predict\<^sub>F k \<G> {x}"
       using Scan\<^sub>F.prems(2,3) Predict\<^sub>F_Un Predict\<^sub>F_Earley\<^sub>F_bin_step_mono by fastforce
     also have "... = bins bs"
       using Scan\<^sub>F.hyps(3,4) Scan\<^sub>F.prems(1) is_terminal_nonterminal wf_earley_input_elim
@@ -1798,25 +1800,25 @@ next
     finally show ?thesis
       using Scan\<^sub>F.hyps(5) Scan\<^sub>F.prems(1,2,3) Complete\<^sub>F_Earley\<^sub>F_bin_step_mono by (auto simp: bins_bins_upd wf_earley_input_elim, blast)
   qed
-  ultimately have "Earley\<^sub>F_bin_step k cfg inp (bins ?bs') \<subseteq> bins (Earley\<^sub>L_bin' k cfg inp ?bs' (i+1))"
+  ultimately have "Earley\<^sub>F_bin_step k \<G> \<omega> (bins ?bs') \<subseteq> bins (Earley\<^sub>L_bin' k \<G> \<omega> ?bs' (i+1))"
     using Scan\<^sub>F.IH Scan\<^sub>F.prems Scan\<^sub>F.hyps(5) sound wf Earley\<^sub>F_bin_step_def bins_upto_sub_bins wf_earley_input_elim
       bins_bins_upd by (metis UnE add_mono1 le_supI)
   thus ?case
     using Earley\<^sub>F_bin_step_sub_mono Earley\<^sub>L_bin'_simps(3) Scan\<^sub>F.hyps Scan\<^sub>F.prems(1) wf_earley_input_elim bins_bins_upd
     by (smt (verit, ccfv_SIG) add_mono1 sup.cobounded1 sup.coboundedI2 sup.orderE)
 next
-  case (Pass k cfg inp bs i x a)
+  case (Pass k \<G> \<omega> bs i x a)
   have x: "x \<in> set (items (bs ! k))"
     using Pass.hyps(1,2) by auto
-  have "Scan\<^sub>F k inp (bins_upto bs k (i + 1)) \<subseteq> bins bs"
+  have "Scan\<^sub>F k \<omega> (bins_upto bs k (i + 1)) \<subseteq> bins bs"
     using Scan\<^sub>F_def Pass.hyps(5) by auto
-  moreover have "Predict\<^sub>F k cfg (bins_upto bs k (i + 1)) \<subseteq> bins bs"
+  moreover have "Predict\<^sub>F k \<G> (bins_upto bs k (i + 1)) \<subseteq> bins bs"
   proof -
-    have "Predict\<^sub>F k cfg (bins_upto bs k (i + 1)) = Predict\<^sub>F k cfg (bins_upto bs k i \<union> {items (bs ! k) ! i})"
+    have "Predict\<^sub>F k \<G> (bins_upto bs k (i + 1)) = Predict\<^sub>F k \<G> (bins_upto bs k i \<union> {items (bs ! k) ! i})"
       using bins_upto_Suc_Un Pass.hyps(1) by (metis items_def length_map not_le_imp_less)
-    also have "... = Predict\<^sub>F k cfg (bins_upto bs k i \<union> {x})"
+    also have "... = Predict\<^sub>F k \<G> (bins_upto bs k i \<union> {x})"
       using Pass.hyps(1,2,5) nth_idem_bins_upd bins_upto_kth_nth_idem by simp
-    also have "... \<subseteq> bins bs \<union> Predict\<^sub>F k cfg {x}"
+    also have "... \<subseteq> bins bs \<union> Predict\<^sub>F k \<G> {x}"
       using Pass.prems(2) Predict\<^sub>F_Un Predict\<^sub>F_Earley\<^sub>F_bin_step_mono by blast
     also have "... = bins bs"
       using Pass.hyps(3,4) Pass.prems(1) is_terminal_nonterminal wf_earley_input_elim
@@ -1835,49 +1837,49 @@ next
     finally show ?thesis
       using Pass.prems(1,2) Complete\<^sub>F_Earley\<^sub>F_bin_step_mono wf_earley_input_elim by blast
   qed
-  ultimately have "Earley\<^sub>F_bin_step k cfg inp (bins bs) \<subseteq> bins (Earley\<^sub>L_bin' k cfg inp bs (i+1))"
+  ultimately have "Earley\<^sub>F_bin_step k \<G> \<omega> (bins bs) \<subseteq> bins (Earley\<^sub>L_bin' k \<G> \<omega> bs (i+1))"
     using Pass.IH Pass.prems Earley\<^sub>F_bin_step_def bins_upto_sub_bins wf_earley_input_elim
     by (metis le_sup_iff)
   thus ?case
     using bins_bins_upd Pass.hyps Pass.prems by simp
 next
-  case (Predict\<^sub>F k cfg inp bs i x a)
-  let ?bs' = "bins_upd bs k (Predict\<^sub>L k cfg a)"
-  have "k \<ge> length inp \<or> \<not> inp!k = a"
+  case (Predict\<^sub>F k \<G> \<omega> bs i x a)
+  let ?bs' = "bins_upd bs k (Predict\<^sub>L k \<G> a)"
+  have "k \<ge> length \<omega> \<or> \<not> \<omega>!k = a"
     using Predict\<^sub>F.hyps(4) Predict\<^sub>F.prems(4) is_word_is_terminal leI by blast
   have x: "x \<in> set (items (bs ! k))"
     using Predict\<^sub>F.hyps(1,2) by auto
-  hence sound: "\<forall>x \<in> set (items(Predict\<^sub>L k cfg a)). sound_item cfg inp x"
+  hence sound: "\<forall>x \<in> set (items(Predict\<^sub>L k \<G> a)). sound_item \<G> \<omega> x"
     using sound_Predict\<^sub>L Predict\<^sub>F.hyps(3) Predict\<^sub>F.prems wf_earley_input_elim wf_bins_impl_wf_items by fast
-  have wf: "(k, cfg, inp, ?bs') \<in> wf_earley_input"
+  have wf: "(k, \<G>, \<omega>, ?bs') \<in> wf_earley_input"
     using Predict\<^sub>F.hyps Predict\<^sub>F.prems(1) wf_earley_input_Predict\<^sub>L by metis
   have len: "i < length (items (?bs' ! k))"
     using length_nth_bin_bins_upd Predict\<^sub>F.hyps(1)
     by (metis dual_order.strict_trans1 items_def length_map linorder_not_less)
-  have "Scan\<^sub>F k inp (bins_upto ?bs' k (i + 1)) \<subseteq> bins ?bs'"
+  have "Scan\<^sub>F k \<omega> (bins_upto ?bs' k (i + 1)) \<subseteq> bins ?bs'"
   proof -
-    have "Scan\<^sub>F k inp (bins_upto ?bs' k (i + 1)) = Scan\<^sub>F k inp (bins_upto ?bs' k i \<union> {items (?bs' ! k) ! i})"
+    have "Scan\<^sub>F k \<omega> (bins_upto ?bs' k (i + 1)) = Scan\<^sub>F k \<omega> (bins_upto ?bs' k i \<union> {items (?bs' ! k) ! i})"
       using Predict\<^sub>F.hyps(1) bins_upto_Suc_Un by (metis items_def len length_map)
-    also have "... = Scan\<^sub>F k inp (bins_upto bs k i \<union> {x})"
+    also have "... = Scan\<^sub>F k \<omega> (bins_upto bs k i \<union> {x})"
       using Predict\<^sub>F.hyps(1,2) Predict\<^sub>F.prems(1) items_nth_idem_bins_upd bins_upto_kth_nth_idem wf_earley_input_elim
       by (metis dual_order.refl items_def length_map not_le_imp_less)
-    also have "... \<subseteq> bins bs \<union> Scan\<^sub>F k inp {x}"
+    also have "... \<subseteq> bins bs \<union> Scan\<^sub>F k \<omega> {x}"
       using Predict\<^sub>F.prems(2,3) Scan\<^sub>F_Un Scan\<^sub>F_Earley\<^sub>F_bin_step_mono by fastforce
     also have "... = bins bs"
-      using Predict\<^sub>F.hyps(3) \<open>length inp \<le> k \<or> inp ! k \<noteq> a\<close> by (auto simp: Scan\<^sub>F_def bin_def)
+      using Predict\<^sub>F.hyps(3) \<open>length \<omega> \<le> k \<or> \<omega> ! k \<noteq> a\<close> by (auto simp: Scan\<^sub>F_def bin_def)
     finally show ?thesis
       using Predict\<^sub>F.prems(1) wf_earley_input_elim bins_bins_upd by blast
   qed
-  moreover have "Predict\<^sub>F k cfg (bins_upto ?bs' k (i + 1)) \<subseteq> bins ?bs'"
+  moreover have "Predict\<^sub>F k \<G> (bins_upto ?bs' k (i + 1)) \<subseteq> bins ?bs'"
   proof -
-    have "Predict\<^sub>F k cfg (bins_upto ?bs' k (i + 1)) = Predict\<^sub>F k cfg (bins_upto ?bs' k i \<union> {items (?bs' ! k) ! i})"
+    have "Predict\<^sub>F k \<G> (bins_upto ?bs' k (i + 1)) = Predict\<^sub>F k \<G> (bins_upto ?bs' k i \<union> {items (?bs' ! k) ! i})"
       using Predict\<^sub>F.hyps(1) bins_upto_Suc_Un by (metis items_def len length_map)
-    also have "... = Predict\<^sub>F k cfg (bins_upto bs k i \<union> {x})"
+    also have "... = Predict\<^sub>F k \<G> (bins_upto bs k i \<union> {x})"
       using Predict\<^sub>F.hyps(1,2) Predict\<^sub>F.prems(1) items_nth_idem_bins_upd bins_upto_kth_nth_idem wf_earley_input_elim
       by (metis dual_order.refl items_def length_map not_le_imp_less)
-    also have "... \<subseteq> bins bs \<union> Predict\<^sub>F k cfg {x}"
+    also have "... \<subseteq> bins bs \<union> Predict\<^sub>F k \<G> {x}"
       using Predict\<^sub>F.prems(2,3) Predict\<^sub>F_Un Predict\<^sub>F_Earley\<^sub>F_bin_step_mono by fastforce
-    also have "... = bins bs \<union> set (items (Predict\<^sub>L k cfg a))"
+    also have "... = bins bs \<union> set (items (Predict\<^sub>L k \<G> a))"
       using Predict\<^sub>F.hyps Predict\<^sub>F.prems(1-3) wf_earley_input_elim
       apply (auto simp: Predict\<^sub>F_def Predict\<^sub>L_def bin_def items_def)
       using wf_bins_kth_bin x by blast
@@ -1900,22 +1902,22 @@ next
     finally show ?thesis
       using bins_bins_upd Predict\<^sub>F.prems(1,2,3) wf_earley_input_elim by (metis Un_upper1 dual_order.trans)
   qed
-  ultimately have "Earley\<^sub>F_bin_step k cfg inp (bins ?bs') \<subseteq> bins (Earley\<^sub>L_bin' k cfg inp ?bs' (i+1))"
+  ultimately have "Earley\<^sub>F_bin_step k \<G> \<omega> (bins ?bs') \<subseteq> bins (Earley\<^sub>L_bin' k \<G> \<omega> ?bs' (i+1))"
     using Predict\<^sub>F.IH Predict\<^sub>F.prems sound wf Earley\<^sub>F_bin_step_def bins_upto_sub_bins
       bins_bins_upd wf_earley_input_elim by (metis UnE le_supI)
-  hence "Earley\<^sub>F_bin_step k cfg inp (bins ?bs') \<subseteq> bins (Earley\<^sub>L_bin' k cfg inp bs i)"
+  hence "Earley\<^sub>F_bin_step k \<G> \<omega> (bins ?bs') \<subseteq> bins (Earley\<^sub>L_bin' k \<G> \<omega> bs i)"
     using Predict\<^sub>F.hyps Earley\<^sub>L_bin'_simps(5) by simp
-  moreover have "Earley\<^sub>F_bin_step k cfg inp (bins bs) \<subseteq> Earley\<^sub>F_bin_step k cfg inp (bins ?bs')"
+  moreover have "Earley\<^sub>F_bin_step k \<G> \<omega> (bins bs) \<subseteq> Earley\<^sub>F_bin_step k \<G> \<omega> (bins ?bs')"
     using Earley\<^sub>F_bin_step_sub_mono Predict\<^sub>F.prems(1) wf_earley_input_elim bins_bins_upd by (metis Un_upper1)
   ultimately show ?case
     by blast
 qed
 
 lemma Earley\<^sub>F_bin_step_sub_Earley\<^sub>L_bin:
-  assumes "(k, cfg, inp, bs) \<in> wf_earley_input"
-  assumes "Earley\<^sub>F_bin_step k cfg inp (bins_upto bs k 0) \<subseteq> bins bs"
-  assumes "\<forall>x \<in> bins bs. sound_item cfg inp x" "is_word cfg inp" "nonempty_derives cfg"
-  shows "Earley\<^sub>F_bin_step k cfg inp (bins bs) \<subseteq> bins (Earley\<^sub>L_bin k cfg inp bs)"
+  assumes "(k, \<G>, \<omega>, bs) \<in> wf_earley_input"
+  assumes "Earley\<^sub>F_bin_step k \<G> \<omega> (bins_upto bs k 0) \<subseteq> bins bs"
+  assumes "\<forall>x \<in> bins bs. sound_item \<G> \<omega> x" "is_word \<G> \<omega>" "nonempty_derives \<G>"
+  shows "Earley\<^sub>F_bin_step k \<G> \<omega> (bins bs) \<subseteq> bins (Earley\<^sub>L_bin k \<G> \<omega> bs)"
   using assms Earley\<^sub>F_bin_step_sub_Earley\<^sub>L_bin' Earley\<^sub>L_bin_def by metis
 
 lemma bins_eq_items_Complete\<^sub>L:
@@ -1931,82 +1933,82 @@ proof -
 qed
 
 lemma Earley\<^sub>L_bin'_bins_eq:
-  assumes "(k, cfg, inp, as) \<in> wf_earley_input"
-  assumes "bins_eq_items as bs" "wf_bins cfg inp as"
-  shows "bins_eq_items (Earley\<^sub>L_bin' k cfg inp as i) (Earley\<^sub>L_bin' k cfg inp bs i)"
+  assumes "(k, \<G>, \<omega>, as) \<in> wf_earley_input"
+  assumes "bins_eq_items as bs" "wf_bins \<G> \<omega> as"
+  shows "bins_eq_items (Earley\<^sub>L_bin' k \<G> \<omega> as i) (Earley\<^sub>L_bin' k \<G> \<omega> bs i)"
   using assms
 proof (induction i arbitrary: bs rule: Earley\<^sub>L_bin'_induct[OF assms(1), case_names Base Complete\<^sub>F Scan\<^sub>F Pass Predict\<^sub>F])
-  case (Base k cfg inp as i)
-  have "Earley\<^sub>L_bin' k cfg inp as i = as"
+  case (Base k \<G> \<omega> as i)
+  have "Earley\<^sub>L_bin' k \<G> \<omega> as i = as"
     by (simp add: Base.hyps)
-  moreover have "Earley\<^sub>L_bin' k cfg inp bs i = bs"
+  moreover have "Earley\<^sub>L_bin' k \<G> \<omega> bs i = bs"
     using Base.hyps Base.prems(1,2) unfolding bins_eq_items_def
     by (metis Earley\<^sub>L_bin'_simps(1) length_map nth_map wf_earley_input_elim)
   ultimately show ?case
     using Base.prems(2) by presburger
 next
-  case (Complete\<^sub>F k cfg inp as i x)
+  case (Complete\<^sub>F k \<G> \<omega> as i x)
   let ?as' = "bins_upd as k (Complete\<^sub>L k x as i)"
   let ?bs' = "bins_upd bs k (Complete\<^sub>L k x bs i)"
   have k: "k < length as"
     using Complete\<^sub>F.prems(1) wf_earley_input_elim by blast
-  hence wf_x: "wf_item cfg inp x"
+  hence wf_x: "wf_item \<G> \<omega> x"
     using Complete\<^sub>F.hyps(1,2) Complete\<^sub>F.prems(3) wf_bins_kth_bin by fastforce
-  have "(k, cfg, inp, ?as') \<in> wf_earley_input"
+  have "(k, \<G>, \<omega>, ?as') \<in> wf_earley_input"
     using Complete\<^sub>F.hyps Complete\<^sub>F.prems(1) wf_earley_input_Complete\<^sub>L by blast
   moreover have "bins_eq_items ?as' ?bs'"
     using Complete\<^sub>F.hyps(1,2) Complete\<^sub>F.prems(2,3) bins_eq_items_dist_bins_upd bins_eq_items_Complete\<^sub>L
       k wf_x wf_bins_kth_bin wf_item_def by (metis dual_order.strict_trans2 leI nth_mem)
-  ultimately have "bins_eq_items (Earley\<^sub>L_bin' k cfg inp ?as' (i + 1)) (Earley\<^sub>L_bin' k cfg inp ?bs' (i + 1))"
+  ultimately have "bins_eq_items (Earley\<^sub>L_bin' k \<G> \<omega> ?as' (i + 1)) (Earley\<^sub>L_bin' k \<G> \<omega> ?bs' (i + 1))"
     using Complete\<^sub>F.IH wf_earley_input_elim by blast
-  moreover have "Earley\<^sub>L_bin' k cfg inp as i = Earley\<^sub>L_bin' k cfg inp ?as' (i+1)"
+  moreover have "Earley\<^sub>L_bin' k \<G> \<omega> as i = Earley\<^sub>L_bin' k \<G> \<omega> ?as' (i+1)"
     using Complete\<^sub>F.hyps by simp
-  moreover have "Earley\<^sub>L_bin' k cfg inp bs i = Earley\<^sub>L_bin' k cfg inp ?bs' (i+1)"
+  moreover have "Earley\<^sub>L_bin' k \<G> \<omega> bs i = Earley\<^sub>L_bin' k \<G> \<omega> ?bs' (i+1)"
     using Complete\<^sub>F.hyps Complete\<^sub>F.prems unfolding bins_eq_items_def
     by (metis Earley\<^sub>L_bin'_simps(2) map_eq_imp_length_eq nth_map wf_earley_input_elim)
   ultimately show ?case
     by argo
 next
-  case (Scan\<^sub>F k cfg inp as i x a)
-  let ?as' = "bins_upd as (k+1) (Scan\<^sub>L k inp a x i)"
-  let ?bs' = "bins_upd bs (k+1) (Scan\<^sub>L k inp a x i)"
-  have "(k, cfg, inp, ?as') \<in> wf_earley_input"
+  case (Scan\<^sub>F k \<G> \<omega> as i x a)
+  let ?as' = "bins_upd as (k+1) (Scan\<^sub>L k \<omega> a x i)"
+  let ?bs' = "bins_upd bs (k+1) (Scan\<^sub>L k \<omega> a x i)"
+  have "(k, \<G>, \<omega>, ?as') \<in> wf_earley_input"
     using Scan\<^sub>F.hyps Scan\<^sub>F.prems(1) wf_earley_input_Scan\<^sub>L by fast
   moreover have "bins_eq_items ?as' ?bs'"
     using Scan\<^sub>F.hyps(5) Scan\<^sub>F.prems(1,2) bins_eq_items_dist_bins_upd add_mono1 wf_earley_input_elim by metis
-  ultimately have "bins_eq_items (Earley\<^sub>L_bin' k cfg inp ?as' (i + 1)) (Earley\<^sub>L_bin' k cfg inp ?bs' (i + 1))"
+  ultimately have "bins_eq_items (Earley\<^sub>L_bin' k \<G> \<omega> ?as' (i + 1)) (Earley\<^sub>L_bin' k \<G> \<omega> ?bs' (i + 1))"
     using Scan\<^sub>F.IH wf_earley_input_elim by blast
-  moreover have "Earley\<^sub>L_bin' k cfg inp as i = Earley\<^sub>L_bin' k cfg inp ?as' (i+1)"
+  moreover have "Earley\<^sub>L_bin' k \<G> \<omega> as i = Earley\<^sub>L_bin' k \<G> \<omega> ?as' (i+1)"
     using Scan\<^sub>F.hyps by simp
-  moreover have "Earley\<^sub>L_bin' k cfg inp bs i = Earley\<^sub>L_bin' k cfg inp ?bs' (i+1)"
+  moreover have "Earley\<^sub>L_bin' k \<G> \<omega> bs i = Earley\<^sub>L_bin' k \<G> \<omega> ?bs' (i+1)"
     using Scan\<^sub>F.hyps Scan\<^sub>F.prems unfolding bins_eq_items_def
     by (smt (verit, ccfv_threshold) Earley\<^sub>L_bin'_simps(3) length_map nth_map wf_earley_input_elim)
   ultimately show ?case
     by argo
 next
-  case (Pass k cfg inp as i x a)
-  have "bins_eq_items (Earley\<^sub>L_bin' k cfg inp as (i + 1)) (Earley\<^sub>L_bin' k cfg inp bs (i + 1))"
+  case (Pass k \<G> \<omega> as i x a)
+  have "bins_eq_items (Earley\<^sub>L_bin' k \<G> \<omega> as (i + 1)) (Earley\<^sub>L_bin' k \<G> \<omega> bs (i + 1))"
     using Pass.prems Pass.IH by blast
-  moreover have "Earley\<^sub>L_bin' k cfg inp as i = Earley\<^sub>L_bin' k cfg inp as (i+1)"
+  moreover have "Earley\<^sub>L_bin' k \<G> \<omega> as i = Earley\<^sub>L_bin' k \<G> \<omega> as (i+1)"
     using Pass.hyps by simp
-  moreover have "Earley\<^sub>L_bin' k cfg inp bs i = Earley\<^sub>L_bin' k cfg inp bs (i+1)"
+  moreover have "Earley\<^sub>L_bin' k \<G> \<omega> bs i = Earley\<^sub>L_bin' k \<G> \<omega> bs (i+1)"
     using Pass.hyps Pass.prems unfolding bins_eq_items_def
     by (metis Earley\<^sub>L_bin'_simps(4) map_eq_imp_length_eq nth_map wf_earley_input_elim)
   ultimately show ?case
     by argo
 next
-  case (Predict\<^sub>F k cfg inp as i x a)
-  let ?as' = "bins_upd as k (Predict\<^sub>L k cfg a)"
-  let ?bs' = "bins_upd bs k (Predict\<^sub>L k cfg a)"
-  have "(k, cfg, inp, ?as') \<in> wf_earley_input"
+  case (Predict\<^sub>F k \<G> \<omega> as i x a)
+  let ?as' = "bins_upd as k (Predict\<^sub>L k \<G> a)"
+  let ?bs' = "bins_upd bs k (Predict\<^sub>L k \<G> a)"
+  have "(k, \<G>, \<omega>, ?as') \<in> wf_earley_input"
     using Predict\<^sub>F.hyps Predict\<^sub>F.prems(1) wf_earley_input_Predict\<^sub>L by fast
   moreover have "bins_eq_items ?as' ?bs'"
     using Predict\<^sub>F.prems(1,2) bins_eq_items_dist_bins_upd wf_earley_input_elim by blast
-  ultimately have "bins_eq_items (Earley\<^sub>L_bin' k cfg inp ?as' (i + 1)) (Earley\<^sub>L_bin' k cfg inp ?bs' (i + 1))"
+  ultimately have "bins_eq_items (Earley\<^sub>L_bin' k \<G> \<omega> ?as' (i + 1)) (Earley\<^sub>L_bin' k \<G> \<omega> ?bs' (i + 1))"
     using Predict\<^sub>F.IH wf_earley_input_elim by blast
-  moreover have "Earley\<^sub>L_bin' k cfg inp as i = Earley\<^sub>L_bin' k cfg inp ?as' (i+1)"
+  moreover have "Earley\<^sub>L_bin' k \<G> \<omega> as i = Earley\<^sub>L_bin' k \<G> \<omega> ?as' (i+1)"
     using Predict\<^sub>F.hyps by simp
-  moreover have "Earley\<^sub>L_bin' k cfg inp bs i = Earley\<^sub>L_bin' k cfg inp ?bs' (i+1)"
+  moreover have "Earley\<^sub>L_bin' k \<G> \<omega> bs i = Earley\<^sub>L_bin' k \<G> \<omega> ?bs' (i+1)"
     using Predict\<^sub>F.hyps Predict\<^sub>F.prems unfolding bins_eq_items_def
     by (metis Earley\<^sub>L_bin'_simps(5) length_map nth_map wf_earley_input_elim)
   ultimately show ?case
@@ -2014,21 +2016,21 @@ next
 qed
 
 lemma Earley\<^sub>L_bin'_idem:
-  assumes "(k, cfg, inp, bs) \<in> wf_earley_input"
-  assumes "i \<le> j" "\<forall>x \<in> bins bs. sound_item cfg inp x" "nonempty_derives cfg"
-  shows "bins (Earley\<^sub>L_bin' k cfg inp (Earley\<^sub>L_bin' k cfg inp bs i) j) = bins (Earley\<^sub>L_bin' k cfg inp bs i)"
+  assumes "(k, \<G>, \<omega>, bs) \<in> wf_earley_input"
+  assumes "i \<le> j" "\<forall>x \<in> bins bs. sound_item \<G> \<omega> x" "nonempty_derives \<G>"
+  shows "bins (Earley\<^sub>L_bin' k \<G> \<omega> (Earley\<^sub>L_bin' k \<G> \<omega> bs i) j) = bins (Earley\<^sub>L_bin' k \<G> \<omega> bs i)"
   using assms
 proof (induction i arbitrary: j rule: Earley\<^sub>L_bin'_induct[OF assms(1), case_names Base Complete\<^sub>F Scan\<^sub>F Pass Predict\<^sub>F])
-  case (Complete\<^sub>F k cfg inp bs i x)
+  case (Complete\<^sub>F k \<G> \<omega> bs i x)
   let ?bs' = "bins_upd bs k (Complete\<^sub>L k x bs i)"
   have x: "x \<in> set (items (bs ! k))"
     using Complete\<^sub>F.hyps(1,2) by auto
-  have wf: "(k, cfg, inp, ?bs') \<in> wf_earley_input"
+  have wf: "(k, \<G>, \<omega>, ?bs') \<in> wf_earley_input"
     using Complete\<^sub>F.hyps Complete\<^sub>F.prems(1) wf_earley_input_Complete\<^sub>L by blast
-  hence "\<forall>x \<in> set (items (Complete\<^sub>L k x bs i)). sound_item cfg inp x"
+  hence "\<forall>x \<in> set (items (Complete\<^sub>L k x bs i)). sound_item \<G> \<omega> x"
     using sound_Complete\<^sub>L Complete\<^sub>F.hyps(3) Complete\<^sub>F.prems wf_earley_input_elim wf_bins_impl_wf_items x
     by (metis dual_order.refl)
-  hence sound: "\<forall>x \<in> bins ?bs'. sound_item cfg inp x"
+  hence sound: "\<forall>x \<in> bins ?bs'. sound_item \<G> \<omega> x"
     by (metis Complete\<^sub>F.prems(1,3) UnE bins_bins_upd wf_earley_input_elim)
   show ?case
   proof cases
@@ -2039,11 +2041,11 @@ proof (induction i arbitrary: j rule: Earley\<^sub>L_bin'_induct[OF assms(1), ca
     assume "\<not> i+1 \<le> j"
     hence "i = j"
       using Complete\<^sub>F.prems(2) by simp
-    have "bins (Earley\<^sub>L_bin' k cfg inp (Earley\<^sub>L_bin' k cfg inp bs i) j) = bins (Earley\<^sub>L_bin' k cfg inp (Earley\<^sub>L_bin' k cfg inp ?bs' (i+1)) j)"
+    have "bins (Earley\<^sub>L_bin' k \<G> \<omega> (Earley\<^sub>L_bin' k \<G> \<omega> bs i) j) = bins (Earley\<^sub>L_bin' k \<G> \<omega> (Earley\<^sub>L_bin' k \<G> \<omega> ?bs' (i+1)) j)"
       using Earley\<^sub>L_bin'_simps(2) Complete\<^sub>F.hyps(1-3) by simp
-    also have "... = bins (Earley\<^sub>L_bin' k cfg inp (Earley\<^sub>L_bin' k cfg inp ?bs' (i+1)) (j+1))"
+    also have "... = bins (Earley\<^sub>L_bin' k \<G> \<omega> (Earley\<^sub>L_bin' k \<G> \<omega> ?bs' (i+1)) (j+1))"
     proof -
-      let ?bs'' = "Earley\<^sub>L_bin' k cfg inp ?bs' (i+1)"
+      let ?bs'' = "Earley\<^sub>L_bin' k \<G> \<omega> ?bs' (i+1)"
       have "length (items (?bs'' ! k)) \<ge> length (items (bs ! k))"
         using length_nth_bin_Earley\<^sub>L_bin' length_nth_bin_bins_upd order_trans wf Complete\<^sub>F.hyps Complete\<^sub>F.prems(1)
         by (smt (verit, ccfv_threshold) Earley\<^sub>L_bin'_simps(2))
@@ -2054,7 +2056,7 @@ proof (induction i arbitrary: j rule: Earley\<^sub>L_bin'_induct[OF assms(1), ca
         by (metis items_def length_map not_le_imp_less)
       hence 1: "x = items (?bs'' ! k) ! j"
         using \<open>i = j\<close> kth_Earley\<^sub>L_bin'_bins Complete\<^sub>F.hyps Complete\<^sub>F.prems(1) Earley\<^sub>L_bin'_simps(2) leI by metis
-      have "bins (Earley\<^sub>L_bin' k cfg inp ?bs'' j) = bins (Earley\<^sub>L_bin' k cfg inp (bins_upd ?bs'' k (Complete\<^sub>L k x ?bs'' i)) (j+1))"
+      have "bins (Earley\<^sub>L_bin' k \<G> \<omega> ?bs'' j) = bins (Earley\<^sub>L_bin' k \<G> \<omega> (bins_upd ?bs'' k (Complete\<^sub>L k x ?bs'' i)) (j+1))"
         using Earley\<^sub>L_bin'_simps(2) 0 1 Complete\<^sub>F.hyps(1,3) Complete\<^sub>F.prems(2) \<open>i = j\<close> by auto
       moreover have "bins_eq_items (bins_upd ?bs'' k (Complete\<^sub>L k x ?bs'' i)) ?bs''"
       proof -
@@ -2084,29 +2086,29 @@ proof (induction i arbitrary: j rule: Earley\<^sub>L_bin'_induct[OF assms(1), ca
         finally show ?thesis
           using bins_eq_items_bins_upd by blast
       qed
-      moreover have "(k, cfg, inp, bins_upd ?bs'' k (Complete\<^sub>L k x ?bs'' i)) \<in> wf_earley_input"
+      moreover have "(k, \<G>, \<omega>, bins_upd ?bs'' k (Complete\<^sub>L k x ?bs'' i)) \<in> wf_earley_input"
         using wf_earley_input_Earley\<^sub>L_bin' wf_earley_input_Complete\<^sub>L Complete\<^sub>F.hyps Complete\<^sub>F.prems(1)
           \<open>length (items (bs ! k)) \<le> length (items (?bs'' ! k))\<close> kth_Earley\<^sub>L_bin'_bins 0 1 by blast
       ultimately show ?thesis
         using Earley\<^sub>L_bin'_bins_eq bins_eq_items_imp_eq_bins wf_earley_input_elim by blast
     qed
-    also have "... = bins (Earley\<^sub>L_bin' k cfg inp ?bs' (i + 1))"
+    also have "... = bins (Earley\<^sub>L_bin' k \<G> \<omega> ?bs' (i + 1))"
       using Complete\<^sub>F.IH[OF wf _ sound Complete\<^sub>F.prems(4)] \<open>i = j\<close> by blast
     finally show ?thesis
       using Complete\<^sub>F.hyps by simp
   qed
 next
-  case (Scan\<^sub>F k cfg inp bs i x a)
-  let ?bs' = "bins_upd bs (k+1) (Scan\<^sub>L k inp a x i)"
+  case (Scan\<^sub>F k \<G> \<omega> bs i x a)
+  let ?bs' = "bins_upd bs (k+1) (Scan\<^sub>L k \<omega> a x i)"
   have x: "x \<in> set (items (bs ! k))"
     using Scan\<^sub>F.hyps(1,2) by auto
-  hence "\<forall>x \<in> set (items (Scan\<^sub>L k inp a x i)). sound_item cfg inp x"
+  hence "\<forall>x \<in> set (items (Scan\<^sub>L k \<omega> a x i)). sound_item \<G> \<omega> x"
     using sound_Scan\<^sub>L Scan\<^sub>F.hyps(3,5) Scan\<^sub>F.prems(1,2,3) wf_earley_input_elim wf_bins_impl_wf_items x
     by (metis dual_order.refl)
-  hence sound: "\<forall>x \<in> bins ?bs'. sound_item cfg inp x"
+  hence sound: "\<forall>x \<in> bins ?bs'. sound_item \<G> \<omega> x"
     using Scan\<^sub>F.hyps(5) Scan\<^sub>F.prems(1,3) bins_bins_upd wf_earley_input_elim
     by (metis UnE add_less_cancel_right)
-  have wf: "(k, cfg, inp, ?bs') \<in> wf_earley_input"
+  have wf: "(k, \<G>, \<omega>, ?bs') \<in> wf_earley_input"
     using Scan\<^sub>F.hyps Scan\<^sub>F.prems(1) wf_earley_input_Scan\<^sub>L by metis
   show ?case
   proof cases
@@ -2117,41 +2119,41 @@ next
     assume "\<not> i+1 \<le> j"
     hence "i = j"
       using Scan\<^sub>F.prems(2) by auto
-    have "bins (Earley\<^sub>L_bin' k cfg inp (Earley\<^sub>L_bin' k cfg inp bs i) j) = bins (Earley\<^sub>L_bin' k cfg inp (Earley\<^sub>L_bin' k cfg inp ?bs' (i+1)) j)"
+    have "bins (Earley\<^sub>L_bin' k \<G> \<omega> (Earley\<^sub>L_bin' k \<G> \<omega> bs i) j) = bins (Earley\<^sub>L_bin' k \<G> \<omega> (Earley\<^sub>L_bin' k \<G> \<omega> ?bs' (i+1)) j)"
       using Scan\<^sub>F.hyps by simp
-    also have "... = bins (Earley\<^sub>L_bin' k cfg inp (Earley\<^sub>L_bin' k cfg inp ?bs' (i+1)) (j+1))"
+    also have "... = bins (Earley\<^sub>L_bin' k \<G> \<omega> (Earley\<^sub>L_bin' k \<G> \<omega> ?bs' (i+1)) (j+1))"
     proof -
-      let ?bs'' = "Earley\<^sub>L_bin' k cfg inp ?bs' (i+1)"
+      let ?bs'' = "Earley\<^sub>L_bin' k \<G> \<omega> ?bs' (i+1)"
       have "length (items (?bs'' ! k)) \<ge> length (items (bs ! k))"
         using length_nth_bin_Earley\<^sub>L_bin' length_nth_bin_bins_upd order_trans Scan\<^sub>F.hyps Scan\<^sub>F.prems(1) Earley\<^sub>L_bin'_simps(3)
         by (smt (verit, ccfv_SIG))
-      hence "bins (Earley\<^sub>L_bin' k cfg inp ?bs'' j) = bins (Earley\<^sub>L_bin' k cfg inp (bins_upd ?bs'' (k+1) (Scan\<^sub>L k inp a x i)) (j+1))"
+      hence "bins (Earley\<^sub>L_bin' k \<G> \<omega> ?bs'' j) = bins (Earley\<^sub>L_bin' k \<G> \<omega> (bins_upd ?bs'' (k+1) (Scan\<^sub>L k \<omega> a x i)) (j+1))"
         using \<open>i = j\<close> kth_Earley\<^sub>L_bin'_bins nth_idem_bins_upd Earley\<^sub>L_bin'_simps(3) Scan\<^sub>F.hyps Scan\<^sub>F.prems(1) by (smt (verit, best) leI le_trans)
-      moreover have "bins_eq_items (bins_upd ?bs'' (k+1) (Scan\<^sub>L k inp a x i)) ?bs''"
+      moreover have "bins_eq_items (bins_upd ?bs'' (k+1) (Scan\<^sub>L k \<omega> a x i)) ?bs''"
       proof -
         have "k+1 < length bs"
           using Scan\<^sub>F.hyps(5) Scan\<^sub>F.prems wf_earley_input_elim by fastforce+
-        hence "set (items (Scan\<^sub>L k inp a x i)) \<subseteq> set (items (?bs' ! (k+1)))"
+        hence "set (items (Scan\<^sub>L k \<omega> a x i)) \<subseteq> set (items (?bs' ! (k+1)))"
           by (simp add: bins_upd_def set_items_bin_upds)
         also have "... \<subseteq> set (items (?bs'' ! (k+1)))"
           using wf nth_bin_sub_Earley\<^sub>L_bin' by blast
         finally show ?thesis
           using bins_eq_items_bins_upd by blast
       qed
-      moreover have "(k, cfg, inp, bins_upd ?bs'' (k+1) (Scan\<^sub>L k inp a x i)) \<in> wf_earley_input"
+      moreover have "(k, \<G>, \<omega>, bins_upd ?bs'' (k+1) (Scan\<^sub>L k \<omega> a x i)) \<in> wf_earley_input"
         using wf_earley_input_Earley\<^sub>L_bin' wf_earley_input_Scan\<^sub>L Scan\<^sub>F.hyps Scan\<^sub>F.prems(1)
           \<open>length (items (bs ! k)) \<le> length (items (?bs'' ! k))\<close> kth_Earley\<^sub>L_bin'_bins
         by (smt (verit, ccfv_SIG) Earley\<^sub>L_bin'_simps(3) linorder_not_le order.trans)
       ultimately show ?thesis
         using Earley\<^sub>L_bin'_bins_eq bins_eq_items_imp_eq_bins wf_earley_input_elim by blast
     qed
-    also have "... = bins (Earley\<^sub>L_bin' k cfg inp ?bs' (i + 1))"
+    also have "... = bins (Earley\<^sub>L_bin' k \<G> \<omega> ?bs' (i + 1))"
       using \<open>i = j\<close> Scan\<^sub>F.IH Scan\<^sub>F.prems Scan\<^sub>F.hyps sound wf_earley_input_Scan\<^sub>L by fast
     finally show ?thesis
       using Scan\<^sub>F.hyps by simp
   qed
 next
-  case (Pass k cfg inp bs i x a)
+  case (Pass k \<G> \<omega> bs i x a)
   show ?case
   proof cases
     assume "i+1 \<le> j"
@@ -2163,15 +2165,15 @@ next
       using Pass Earley\<^sub>L_bin'_simps(1,4) kth_Earley\<^sub>L_bin'_bins by (metis Suc_eq_plus1 Suc_leI antisym_conv2 not_le_imp_less)
   qed
 next
-  case (Predict\<^sub>F k cfg inp bs i x a)
-  let ?bs' = "bins_upd bs k (Predict\<^sub>L k cfg a)"
+  case (Predict\<^sub>F k \<G> \<omega> bs i x a)
+  let ?bs' = "bins_upd bs k (Predict\<^sub>L k \<G> a)"
   have x: "x \<in> set (items (bs ! k))"
     using Predict\<^sub>F.hyps(1,2) by auto
-  hence "\<forall>x \<in> set (items(Predict\<^sub>L k cfg a)). sound_item cfg inp x"
+  hence "\<forall>x \<in> set (items(Predict\<^sub>L k \<G> a)). sound_item \<G> \<omega> x"
     using sound_Predict\<^sub>L Predict\<^sub>F.hyps(3) Predict\<^sub>F.prems wf_earley_input_elim wf_bins_impl_wf_items by fast
-  hence sound: "\<forall>x \<in> bins ?bs'. sound_item cfg inp x"
+  hence sound: "\<forall>x \<in> bins ?bs'. sound_item \<G> \<omega> x"
     using Predict\<^sub>F.prems(1,3) UnE bins_bins_upd wf_earley_input_elim by metis
-  have wf: "(k, cfg, inp, ?bs') \<in> wf_earley_input"
+  have wf: "(k, \<G>, \<omega>, ?bs') \<in> wf_earley_input"
     using Predict\<^sub>F.hyps Predict\<^sub>F.prems(1) wf_earley_input_Predict\<^sub>L by metis
   have len: "i < length (items (?bs' ! k))"
     using length_nth_bin_bins_upd Predict\<^sub>F.hyps(1) Orderings.preorder_class.dual_order.strict_trans1 linorder_not_less
@@ -2185,36 +2187,36 @@ next
     assume "\<not> i+1 \<le> j"
     hence "i = j"
       using Predict\<^sub>F.prems(2) by auto
-    have "bins (Earley\<^sub>L_bin' k cfg inp (Earley\<^sub>L_bin' k cfg inp bs i) j) = bins (Earley\<^sub>L_bin' k cfg inp (Earley\<^sub>L_bin' k cfg inp ?bs' (i+1)) j)"
+    have "bins (Earley\<^sub>L_bin' k \<G> \<omega> (Earley\<^sub>L_bin' k \<G> \<omega> bs i) j) = bins (Earley\<^sub>L_bin' k \<G> \<omega> (Earley\<^sub>L_bin' k \<G> \<omega> ?bs' (i+1)) j)"
       using Predict\<^sub>F.hyps by simp
-    also have "... = bins (Earley\<^sub>L_bin' k cfg inp (Earley\<^sub>L_bin' k cfg inp ?bs' (i+1)) (j+1))"
+    also have "... = bins (Earley\<^sub>L_bin' k \<G> \<omega> (Earley\<^sub>L_bin' k \<G> \<omega> ?bs' (i+1)) (j+1))"
     proof -
-      let ?bs'' = "Earley\<^sub>L_bin' k cfg inp ?bs' (i+1)"
+      let ?bs'' = "Earley\<^sub>L_bin' k \<G> \<omega> ?bs' (i+1)"
       have "length (items (?bs'' ! k)) \<ge> length (items (bs ! k))"
         using length_nth_bin_Earley\<^sub>L_bin' length_nth_bin_bins_upd order_trans wf
         by (metis (no_types, lifting) items_def length_map)
-      hence "bins (Earley\<^sub>L_bin' k cfg inp ?bs'' j) = bins (Earley\<^sub>L_bin' k cfg inp (bins_upd ?bs'' k (Predict\<^sub>L k cfg a)) (j+1))"
+      hence "bins (Earley\<^sub>L_bin' k \<G> \<omega> ?bs'' j) = bins (Earley\<^sub>L_bin' k \<G> \<omega> (bins_upd ?bs'' k (Predict\<^sub>L k \<G> a)) (j+1))"
         using \<open>i = j\<close> kth_Earley\<^sub>L_bin'_bins nth_idem_bins_upd Earley\<^sub>L_bin'_simps(5) Predict\<^sub>F.hyps Predict\<^sub>F.prems(1) length_bins_Earley\<^sub>L_bin'
           wf_bins_Earley\<^sub>L_bin' wf_bins_kth_bin wf_item_def x by (smt (verit, ccfv_SIG) linorder_not_le order.trans)
-      moreover have "bins_eq_items (bins_upd ?bs'' k (Predict\<^sub>L k cfg a)) ?bs''"
+      moreover have "bins_eq_items (bins_upd ?bs'' k (Predict\<^sub>L k \<G> a)) ?bs''"
       proof -
         have "k < length bs"
           using wf_earley_input_elim[OF Predict\<^sub>F.prems(1)] by blast
-        hence "set (items (Predict\<^sub>L k cfg a)) \<subseteq> set (items (?bs' ! k))"
+        hence "set (items (Predict\<^sub>L k \<G> a)) \<subseteq> set (items (?bs' ! k))"
           by (simp add: bins_upd_def set_items_bin_upds)
         also have "... \<subseteq> set (items (?bs'' ! k))"
           using wf nth_bin_sub_Earley\<^sub>L_bin' by blast
         finally show ?thesis
           using bins_eq_items_bins_upd by blast
       qed
-      moreover have "(k, cfg, inp, bins_upd ?bs'' k (Predict\<^sub>L k cfg a)) \<in> wf_earley_input"
+      moreover have "(k, \<G>, \<omega>, bins_upd ?bs'' k (Predict\<^sub>L k \<G> a)) \<in> wf_earley_input"
         using wf_earley_input_Earley\<^sub>L_bin' wf_earley_input_Predict\<^sub>L Predict\<^sub>F.hyps Predict\<^sub>F.prems(1)
           \<open>length (items (bs ! k)) \<le> length (items (?bs'' ! k))\<close> kth_Earley\<^sub>L_bin'_bins
         by (smt (verit, best) Earley\<^sub>L_bin'_simps(5) dual_order.trans not_le_imp_less)
       ultimately show ?thesis
         using Earley\<^sub>L_bin'_bins_eq bins_eq_items_imp_eq_bins wf_earley_input_elim by blast
     qed
-    also have "... = bins (Earley\<^sub>L_bin' k cfg inp ?bs' (i + 1))"
+    also have "... = bins (Earley\<^sub>L_bin' k \<G> \<omega> ?bs' (i + 1))"
       using \<open>i = j\<close> Predict\<^sub>F.IH Predict\<^sub>F.prems sound wf by (metis order_refl)
     finally show ?thesis
       using Predict\<^sub>F.hyps by simp
@@ -2222,16 +2224,16 @@ next
 qed simp
 
 lemma Earley\<^sub>L_bin_idem:
-  assumes "(k, cfg, inp, bs) \<in> wf_earley_input"
-  assumes "\<forall>x \<in> bins bs. sound_item cfg inp x" "nonempty_derives cfg"
-  shows "bins (Earley\<^sub>L_bin k cfg inp (Earley\<^sub>L_bin k cfg inp bs)) = bins (Earley\<^sub>L_bin k cfg inp bs)"
+  assumes "(k, \<G>, \<omega>, bs) \<in> wf_earley_input"
+  assumes "\<forall>x \<in> bins bs. sound_item \<G> \<omega> x" "nonempty_derives \<G>"
+  shows "bins (Earley\<^sub>L_bin k \<G> \<omega> (Earley\<^sub>L_bin k \<G> \<omega> bs)) = bins (Earley\<^sub>L_bin k \<G> \<omega> bs)"
   using assms Earley\<^sub>L_bin'_idem Earley\<^sub>L_bin_def le0 by metis
 
 lemma funpower_Earley\<^sub>F_bin_step_sub_Earley\<^sub>L_bin:
-  assumes "(k, cfg, inp, bs) \<in> wf_earley_input"
-  assumes "Earley\<^sub>F_bin_step k cfg inp (bins_upto bs k 0) \<subseteq> bins bs" "\<forall>x \<in> bins bs. sound_item cfg inp x"
-  assumes "is_word cfg inp" "nonempty_derives cfg"
-  shows "funpower (Earley\<^sub>F_bin_step k cfg inp) n (bins bs) \<subseteq> bins (Earley\<^sub>L_bin k cfg inp bs)"
+  assumes "(k, \<G>, \<omega>, bs) \<in> wf_earley_input"
+  assumes "Earley\<^sub>F_bin_step k \<G> \<omega> (bins_upto bs k 0) \<subseteq> bins bs" "\<forall>x \<in> bins bs. sound_item \<G> \<omega> x"
+  assumes "is_word \<G> \<omega>" "nonempty_derives \<G>"
+  shows "funpower (Earley\<^sub>F_bin_step k \<G> \<omega>) n (bins bs) \<subseteq> bins (Earley\<^sub>L_bin k \<G> \<omega> bs)"
   using assms
 proof (induction n)
   case 0
@@ -2239,33 +2241,33 @@ proof (induction n)
     using Earley\<^sub>L_bin'_mono Earley\<^sub>L_bin_def by (simp add: Earley\<^sub>L_bin'_mono Earley\<^sub>L_bin_def)
 next
   case (Suc n)
-  have 0: "Earley\<^sub>F_bin_step k cfg inp (bins_upto (Earley\<^sub>L_bin k cfg inp bs) k 0) \<subseteq> bins (Earley\<^sub>L_bin k cfg inp bs)"
+  have 0: "Earley\<^sub>F_bin_step k \<G> \<omega> (bins_upto (Earley\<^sub>L_bin k \<G> \<omega> bs) k 0) \<subseteq> bins (Earley\<^sub>L_bin k \<G> \<omega> bs)"
     using Earley\<^sub>L_bin'_mono bins_upto_k0_Earley\<^sub>L_bin'_eq assms(1,2) Earley\<^sub>L_bin_def order_trans
     by (metis (no_types, lifting))
-  have "funpower (Earley\<^sub>F_bin_step k cfg inp) (Suc n) (bins bs) \<subseteq> Earley\<^sub>F_bin_step k cfg inp (bins (Earley\<^sub>L_bin k cfg inp bs))"
+  have "funpower (Earley\<^sub>F_bin_step k \<G> \<omega>) (Suc n) (bins bs) \<subseteq> Earley\<^sub>F_bin_step k \<G> \<omega> (bins (Earley\<^sub>L_bin k \<G> \<omega> bs))"
     using Earley\<^sub>F_bin_step_sub_mono Suc by (metis funpower.simps(2))
-  also have "... \<subseteq> bins (Earley\<^sub>L_bin k cfg inp (Earley\<^sub>L_bin k cfg inp bs))"
+  also have "... \<subseteq> bins (Earley\<^sub>L_bin k \<G> \<omega> (Earley\<^sub>L_bin k \<G> \<omega> bs))"
     using Earley\<^sub>F_bin_step_sub_Earley\<^sub>L_bin Suc.prems wf_bins_Earley\<^sub>L_bin sound_Earley\<^sub>L_bin 0 wf_earley_input_Earley\<^sub>L_bin by blast
-  also have "... \<subseteq> bins (Earley\<^sub>L_bin k cfg inp bs)"
+  also have "... \<subseteq> bins (Earley\<^sub>L_bin k \<G> \<omega> bs)"
     using Earley\<^sub>L_bin_idem Suc.prems by blast
   finally show ?case .
 qed
 
 lemma Earley\<^sub>F_bin_sub_Earley\<^sub>L_bin:
-  assumes "(k, cfg, inp, bs) \<in> wf_earley_input"
-  assumes "Earley\<^sub>F_bin_step k cfg inp (bins_upto bs k 0) \<subseteq> bins bs" "\<forall>x \<in> bins bs. sound_item cfg inp x"
-  assumes "is_word cfg inp" "nonempty_derives cfg"
-  shows "Earley\<^sub>F_bin k cfg inp (bins bs) \<subseteq> bins (Earley\<^sub>L_bin k cfg inp bs)"
+  assumes "(k, \<G>, \<omega>, bs) \<in> wf_earley_input"
+  assumes "Earley\<^sub>F_bin_step k \<G> \<omega> (bins_upto bs k 0) \<subseteq> bins bs" "\<forall>x \<in> bins bs. sound_item \<G> \<omega> x"
+  assumes "is_word \<G> \<omega>" "nonempty_derives \<G>"
+  shows "Earley\<^sub>F_bin k \<G> \<omega> (bins bs) \<subseteq> bins (Earley\<^sub>L_bin k \<G> \<omega> bs)"
   using assms funpower_Earley\<^sub>F_bin_step_sub_Earley\<^sub>L_bin Earley\<^sub>F_bin_def elem_limit_simp by fastforce
 
 lemma Earley\<^sub>F_bins_sub_Earley\<^sub>L_bins:
-  assumes "k \<le> length inp" "wf_\<G> cfg"
-  assumes "is_word cfg inp" "nonempty_derives cfg"
-  shows "Earley\<^sub>F_bins k cfg inp \<subseteq> bins (Earley\<^sub>L_bins k cfg inp)"
+  assumes "k \<le> length \<omega>" "wf_\<G> \<G>"
+  assumes "is_word \<G> \<omega>" "nonempty_derives \<G>"
+  shows "Earley\<^sub>F_bins k \<G> \<omega> \<subseteq> bins (Earley\<^sub>L_bins k \<G> \<omega>)"
   using assms
 proof (induction k)
   case 0
-  hence "Earley\<^sub>F_bin 0 cfg inp (Init\<^sub>F cfg) \<subseteq> bins (Earley\<^sub>L_bin 0 cfg inp (Init\<^sub>L cfg inp))"
+  hence "Earley\<^sub>F_bin 0 \<G> \<omega> (Init\<^sub>F \<G>) \<subseteq> bins (Earley\<^sub>L_bin 0 \<G> \<omega> (Init\<^sub>L \<G> \<omega>))"
     using Earley\<^sub>F_bin_sub_Earley\<^sub>L_bin Init\<^sub>L_eq_Init\<^sub>F length_bins_Init\<^sub>L Init\<^sub>L_eq_Init\<^sub>F sound_Init bins_upto_empty
       Earley\<^sub>F_bin_step_empty bins_upto_sub_bins wf_earley_input_Init\<^sub>L wf_earley_input_elim
     by (smt (verit, ccfv_threshold) Init\<^sub>F_sub_Earley basic_trans_rules(31) sound_Earley wf_bins_impl_wf_items)
@@ -2273,59 +2275,49 @@ proof (induction k)
     by simp
 next
   case (Suc k)
-  have wf: "(Suc k, cfg, inp, Earley\<^sub>L_bins k cfg inp) \<in> wf_earley_input"
+  have wf: "(Suc k, \<G>, \<omega>, Earley\<^sub>L_bins k \<G> \<omega>) \<in> wf_earley_input"
     by (simp add: Suc.prems(1) Suc_leD assms(2) wf_earley_input_intro)
-  have sub: "Earley\<^sub>F_bin_step (Suc k) cfg inp (bins_upto (Earley\<^sub>L_bins k cfg inp) (Suc k) 0) \<subseteq> bins (Earley\<^sub>L_bins k cfg inp)"
+  have sub: "Earley\<^sub>F_bin_step (Suc k) \<G> \<omega> (bins_upto (Earley\<^sub>L_bins k \<G> \<omega>) (Suc k) 0) \<subseteq> bins (Earley\<^sub>L_bins k \<G> \<omega>)"
   proof -
-    have "bin (bins_upto (Earley\<^sub>L_bins k cfg inp) (Suc k) 0) (Suc k) = {}"
+    have "bin (bins_upto (Earley\<^sub>L_bins k \<G> \<omega>) (Suc k) 0) (Suc k) = {}"
       using kth_bin_bins_upto_empty wf Suc.prems wf_earley_input_elim by blast
-    hence "Earley\<^sub>F_bin_step (Suc k) cfg inp (bins_upto (Earley\<^sub>L_bins k cfg inp) (Suc k) 0) = bins_upto (Earley\<^sub>L_bins k cfg inp) (Suc k) 0"
+    hence "Earley\<^sub>F_bin_step (Suc k) \<G> \<omega> (bins_upto (Earley\<^sub>L_bins k \<G> \<omega>) (Suc k) 0) = bins_upto (Earley\<^sub>L_bins k \<G> \<omega>) (Suc k) 0"
       unfolding Earley\<^sub>F_bin_step_def Scan\<^sub>F_def Complete\<^sub>F_def Predict\<^sub>F_def bin_def by blast
-    also have "... \<subseteq> bins (Earley\<^sub>L_bins k cfg inp)"
+    also have "... \<subseteq> bins (Earley\<^sub>L_bins k \<G> \<omega>)"
       using wf Suc.prems bins_upto_sub_bins wf_earley_input_elim by blast
     finally show ?thesis .
   qed
-  have sound: "\<forall>x \<in> bins (Earley\<^sub>L_bins k cfg inp). sound_item cfg inp x"
+  have sound: "\<forall>x \<in> bins (Earley\<^sub>L_bins k \<G> \<omega>). sound_item \<G> \<omega> x"
     using Suc Earley\<^sub>L_bins_sub_Earley\<^sub>F_bins by (metis Suc_leD Earley\<^sub>F_bins_sub_Earley in_mono sound_Earley wf_Earley)
-  have "Earley\<^sub>F_bins (Suc k) cfg inp \<subseteq> Earley\<^sub>F_bin (Suc k) cfg inp (bins (Earley\<^sub>L_bins k cfg inp))"
+  have "Earley\<^sub>F_bins (Suc k) \<G> \<omega> \<subseteq> Earley\<^sub>F_bin (Suc k) \<G> \<omega> (bins (Earley\<^sub>L_bins k \<G> \<omega>))"
     using Suc Earley\<^sub>F_bin_sub_mono by simp
-  also have "... \<subseteq> bins (Earley\<^sub>L_bin (Suc k) cfg inp (Earley\<^sub>L_bins k cfg inp))"
+  also have "... \<subseteq> bins (Earley\<^sub>L_bin (Suc k) \<G> \<omega> (Earley\<^sub>L_bins k \<G> \<omega>))"
     using Earley\<^sub>F_bin_sub_Earley\<^sub>L_bin wf sub sound Suc.prems by fastforce
   finally show ?case
     by simp
 qed
 
 lemma Earley\<^sub>F_sub_Earley\<^sub>L:
-  assumes "wf_\<G> cfg" "is_word cfg inp" "nonempty_derives cfg"
-  shows "Earley\<^sub>F cfg inp \<subseteq> bins (Earley\<^sub>L cfg inp)"
+  assumes "wf_\<G> \<G>" "is_word \<G> \<omega>" "nonempty_derives \<G>"
+  shows "Earley\<^sub>F \<G> \<omega> \<subseteq> bins (Earley\<^sub>L \<G> \<omega>)"
   using assms Earley\<^sub>F_bins_sub_Earley\<^sub>L_bins Earley\<^sub>F_def Earley\<^sub>L_def by (metis le_refl)
+
+theorem completeness_Earley\<^sub>L:
+  assumes "derives \<G> [\<SS> \<G>] \<omega>" "is_word \<G> \<omega>" "wf_\<G> \<G>" "nonempty_derives \<G>"
+  shows "recognizing (bins (Earley\<^sub>L \<G> \<omega>)) \<G> \<omega>"
+  using assms Earley\<^sub>F_sub_Earley\<^sub>L Earley\<^sub>L_sub_Earley\<^sub>F completeness_Earley\<^sub>F by (metis subset_antisym)
 
 
 subsection \<open>Correctness\<close>
 
-definition earley_recognized_it :: "'a bins \<Rightarrow> 'a cfg \<Rightarrow> 'a sentence \<Rightarrow> bool" where
-  "earley_recognized_it I cfg inp = (\<exists>x \<in> set (items (I ! length inp)). is_finished cfg inp x)"
+theorem Earley_eq_Earley\<^sub>L:
+  assumes "wf_\<G> \<G>" "is_word \<G> \<omega>" "nonempty_derives \<G>"
+  shows "Earley \<G> \<omega> = bins (Earley\<^sub>L \<G> \<omega>)"
+  using assms Earley\<^sub>F_sub_Earley\<^sub>L Earley\<^sub>L_sub_Earley\<^sub>F Earley_eq_Earley\<^sub>F by blast
 
-theorem earley_recognized_it_iff_earley_recognized:
-  assumes "wf_\<G> cfg" "is_word cfg inp" "nonempty_derives cfg"
-  shows "earley_recognized_it (Earley\<^sub>L cfg inp) cfg inp \<longleftrightarrow> recognizing (Earley\<^sub>F cfg inp) cfg inp"
-proof -
-  have "earley_recognized_it (Earley\<^sub>L cfg inp) cfg inp = (\<exists>x \<in> set (items ((Earley\<^sub>L cfg inp) ! length inp)). is_finished cfg inp x)"
-    unfolding earley_recognized_it_def by blast
-  also have "... = (\<exists>x \<in> bins (Earley\<^sub>L cfg inp). is_finished cfg inp x)"
-    using is_finished_def kth_bin_sub_bins Earley\<^sub>L_def length_bins_Init\<^sub>L wf_bins_Earley\<^sub>L
-      wf_item_in_kth_bin length_Earley\<^sub>L_bins assms(1)
-    by (smt (verit) le_eq_less_or_eq subset_code(1) wf_earley_input_Earley\<^sub>L_bins wf_earley_input_elim)
-  also have "... = (\<exists>x \<in> Earley\<^sub>F cfg inp. is_finished cfg inp x)"
-    using assms Earley\<^sub>L_sub_Earley\<^sub>F Earley\<^sub>F_sub_Earley\<^sub>L by blast
-  also have "... = recognizing (Earley\<^sub>F cfg inp) cfg inp"
-    unfolding recognizing_def by blast
-  finally show ?thesis .
-qed
-
-corollary correctness_list:
-  assumes "wf_\<G> cfg" "is_word cfg inp" "nonempty_derives cfg"
-  shows "earley_recognized_it (Earley\<^sub>L cfg inp) cfg inp \<longleftrightarrow> derives cfg [\<SS> cfg] inp"
-  by (metis Earley_eq_Earley\<^sub>F assms correctness_Earley earley_recognized_it_iff_earley_recognized)
+theorem correctness_Earley\<^sub>L:
+  assumes "wf_\<G> \<G>" "is_word \<G> \<omega>" "nonempty_derives \<G>"
+  shows "recognizing (bins (Earley\<^sub>L \<G> \<omega>)) \<G> \<omega> \<longleftrightarrow> derives \<G> [\<SS> \<G>] \<omega>"
+  using assms Earley_eq_Earley\<^sub>L correctness_Earley by fastforce
 
 end
